definitely prove that reachability is well-defined

doc/coq/Concrete.v
@@ -71,318 +71,362 @@ Inductive EvalR `{time T} (C : @dy_ctx T) (st : @state T)
 
 #[export] Hint Constructors EvalR : core.
 
+Inductive config {T} :=
+  | Config (C : @dy_ctx T) (st : @state T) (e : tm)
+.
+
 Inductive interpreter_state {T} :=
-  | Pending (C : @dy_ctx T) (st : @state T) (e : tm)
-  | Error (C : @dy_ctx T) (st : @state T) (e : tm) (* Type error *)
-  | Resolved (v : @dy_value T) (st : @state T)
+  | Pending (reached : list (@config T))
+  | Error (reached : list (@config T)) (* Type error *)
+  | Resolved (v : @dy_value T) (st : @state T) (reached : list (@config T))
 .
 
 Fixpoint eval `{time T} (C : @dy_ctx T) (st : @state T) 
-              (e : tm) (FUEL : nat) :=
+              (e : tm) (reached : list config) (FUEL : nat) :=
+  let reached := (Config C st e) :: reached in
   match FUEL with
-  | 0 => Pending C st e
+  | 0 => Pending reached
   | S FUEL' =>
     match e with
     | e_var x =>
       match addr_x C x with
-      | None => Error C st e
-      | Some addr => 
+      | None => Error reached
+      | Some addr =>
         match st with
         | ST mem _ =>
           match mem addr with
-          | None => Pending C st e
-          | Some v => Resolved (EVal v) st
+          | None => Pending reached
+          | Some v => Resolved (EVal v) st reached
           end
         end
       end
     | e_lam x e' =>
-      Resolved (EVal (Closure x e' C)) st
+      Resolved (EVal (Closure x e' C)) st reached
     | e_app e1 e2 =>
-      match eval C st e1 FUEL' with
-      | Resolved (EVal (Closure x e' C_lam)) st_lam =>
-        match eval C st_lam e2 FUEL' with
-        | Resolved (EVal arg) (ST mem t) =>
+      match eval C st e1 reached FUEL' with
+      | Resolved (EVal (Closure x e' C_lam)) st_lam reached' =>
+        match eval C st_lam e2 reached' FUEL' with
+        | Resolved (EVal arg) (ST mem t) reached'' =>
           match eval (C_lam [| dy_c_lam x t ([||]) |]) 
                      (ST (t !-> arg ; mem) 
                          (update C (ST mem t) x arg)) 
-                     e' FUEL' with
-          | Resolved (EVal v) st' => Resolved (EVal v) st'
-          | Resolved _ _ => Error C st e
+                     e' reached'' FUEL' with
+          | Resolved (EVal v) st' reached''' => Resolved (EVal v) st' reached'''
+          | Resolved _ _ reached''' => Error reached'''
           | other => other
           end
-        | Resolved _ _ => Error C st e
+        | Resolved _ _ reached'' => Error reached''
         | other => other
         end
-      | Resolved _ _ => Error C st e
+      | Resolved _ _ reached' => Error reached'
       | other => other
       end
     | e_link m e' =>
-      match eval C st m FUEL' with
-      | Resolved (MVal C_m) st_m =>
-        match eval C_m st_m e' FUEL' with
-        | Resolved v st' => Resolved v st'
+      match eval C st m reached FUEL' with
+      | Resolved (MVal C_m) st_m reached' =>
+        match eval C_m st_m e' reached' FUEL' with
+        | Resolved v st' reached'' => Resolved v st' reached''
         | other => other
         end
-      | Resolved _ _ => Error C st e
+      | Resolved _ _ reached' => Error reached'
       | other => other
       end
-    | m_empty => Resolved (MVal C) st
+    | m_empty => Resolved (MVal C) st reached
     | m_var M =>
       match ctx_M C M with
-      | None => Pending C st e
-      | Some C_M => Resolved (MVal C_M) st
+      | None => Pending reached
+      | Some C_M => Resolved (MVal C_M) st reached
       end
     | m_lete x e m =>
-      match eval C st e FUEL' with
-      | Resolved (EVal v) (ST mem t) =>
+      match eval C st e reached FUEL' with
+      | Resolved (EVal v) (ST mem t) reached' =>
         match eval (C[| dy_c_lete x t ([||]) |]) 
                    (ST (t !-> v ; mem) 
                        (update C (ST mem t) x v)) 
-                   m FUEL' with
-        | Resolved (MVal C') st' => Resolved (MVal C') st'
-        | Resolved _ _ => Error C st e 
+                   m reached' FUEL' with
+        | Resolved (MVal C') st' reached'' => Resolved (MVal C') st' reached''
+        | Resolved _ _ reached'' => Error reached''
         | other => other
         end
-      | Resolved _ _ => Error C st e
+      | Resolved _ _ reached' => Error reached'
       | other => other
       end
     | m_letm M m1 m2 =>
-      match eval C st m1 FUEL' with
-      | Resolved (MVal C') st' =>
+      match eval C st m1 reached FUEL' with
+      | Resolved (MVal C') st' reached' =>
         match eval (C[| dy_c_letm M C' ([||]) |])
-                   st' m2 FUEL' with
-        | Resolved (MVal C'') st'' => Resolved (MVal C'') st''
-        | Resolved _ _ => Error C st e
+                   st' m2 reached' FUEL' with
+        | Resolved (MVal C'') st'' reached'' => Resolved (MVal C'') st'' reached''
+        | Resolved _ _ reached'' => Error reached''
         | other => other
         end
-      | Resolved _ _ => Error C st e
+      | Resolved _ _ reached' => Error reached'
       | other => other
       end
     end
   end.
 
 Lemma relax_fuel :
-  forall `{TIME : time T} (C : @dy_ctx T) st e v st' FUEL FUEL' (LE : FUEL <= FUEL'),
-    eval C st e FUEL = Resolved v st' ->
-    eval C st e FUEL' = Resolved v st'.
+  forall `{TIME : time T} (C : @dy_ctx T) st e l l' v st' FUEL FUEL' (LE : FUEL <= FUEL'),
+    eval C st e l FUEL = Resolved v st' l' ->
+    eval C st e l FUEL' = Resolved v st' l'.
 Proof.
   intros. rename H into H'. rename H0 into H''. rename H1 into H.
-  revert C st e v st' H FUEL' LE.
+  revert C st e l l' v st' H FUEL' LE.
   induction FUEL; intros.
   - inversion H.
   - simpl in H; destruct e; inversion LE; eauto.
-    + remember (eval C st e1 FUEL) as v1.
+    + remember (eval C st e1 (Config C st (e_app e1 e2) :: l) FUEL) as v1.
       destruct v1 as [ | | v1 st1]; inversion H.
       clear H3. destruct v1 as [v1 | ]; inversion H.
       clear H3. destruct v1 as [x v1 C_lam].
-      remember (eval C st1 e2 FUEL) as v2.
+      remember (eval C st1 e2 reached FUEL) as v2.
       destruct v2 as [ | | v2 st2]; inversion H;
       clear H3. destruct v2 as [v2 | ]; inversion H.
       clear H3. destruct st2 as [mem2 t2].
       remember (eval (C_lam [|dy_c_lam x t2 ([||])|]) 
                      (ST (t2 !-> v2; mem2) (update C (ST mem2 t2) x v2))
-                      v1 FUEL) as v3.
+                      v1 reached0 FUEL) as v3.
       destruct v3 as [ | | v3 st3]; inversion H.
       clear H3. destruct v3 as [v3 | ]; inversion H.
       subst. 
-      assert (eval C st e1 m = Resolved (EVal (Closure x v1 C_lam)) st1) as RR1.
+      assert (eval C st e1 (Config C st (e_app e1 e2) :: l) m = Resolved (EVal (Closure x v1 C_lam)) st1 reached) as RR1.
       apply IHFUEL; eauto. nia.
-      assert (eval C st1 e2 m = Resolved (EVal v2) (ST mem2 t2)) as RR2.
+      assert (eval C st1 e2 reached m = Resolved (EVal v2) (ST mem2 t2) reached0) as RR2.
       apply IHFUEL; eauto. nia.
       assert (eval (C_lam [|dy_c_lam x t2 ([||])|])
-                   (ST (t2 !-> v2; mem2) (update C (ST mem2 t2) x v2)) v1 m = 
-              Resolved (EVal v3) st') as RR3.
+                   (ST (t2 !-> v2; mem2) (update C (ST mem2 t2) x v2)) v1 reached0 m = 
+              Resolved (EVal v3) st' l') as RR3.
       apply IHFUEL; eauto. nia.
       simpl. rewrite RR1. rewrite RR2. rewrite RR3. eauto.
-    + remember (eval C st e1 FUEL) as v1.
+    + remember (eval C st e1 (Config C st (e_link e1 e2) :: l) FUEL) as v1.
       destruct v1 as [ | | v1 st1]; inversion H.
       clear H3. destruct v1 as [v1 | ]; inversion H.
-      remember (eval mv st1 e2 FUEL) as v2.
+      remember (eval mv st1 e2 reached FUEL) as v2.
       clear H3. destruct v2 as [ | | v2 st2]; inversion H.
       clear H3. destruct v2 as [v2 | ]; inversion H; subst;
-      assert (eval C st e1 m = Resolved (MVal mv) st1) as RR1;
+      assert (eval C st e1 (Config C st (e_link e1 e2) :: l) m = Resolved (MVal mv) st1 reached) as RR1;
       try (apply IHFUEL; eauto; nia).
-      assert (eval mv st1 e2 m = Resolved (EVal v2) st') as RR2.
+      assert (eval mv st1 e2 reached m = Resolved (EVal v2) st' l') as RR2.
       apply IHFUEL; eauto; nia.
       simpl. rewrite RR1. rewrite RR2. eauto.
-      assert (eval mv st1 e2 m = Resolved (MVal mv0) st') as RR2.
+      assert (eval mv st1 e2 reached m = Resolved (MVal mv0) st' l') as RR2.
       apply IHFUEL; eauto; nia.
       simpl. rewrite RR1. rewrite RR2. eauto.
-    + remember (eval C st e1 FUEL) as v1.
+    + remember (eval C st e1 (Config C st (m_lete x e1 e2) :: l) FUEL) as v1.
       destruct v1 as [ | | v1 st1]; inversion H.
       clear H3. destruct v1 as [v1 | ]; inversion H.
       clear H3. destruct st1 as [mem1 t1].
       remember (eval (C [|dy_c_lete x t1 ([||])|]) 
                      (ST (t1 !-> v1; mem1) (update C (ST mem1 t1) x v1))
-                      e2 FUEL) as v2.
+                      e2 reached FUEL) as v2.
       destruct v2 as [ | | v2 st2]; inversion H.
       clear H3. destruct v2 as [v2 | ]; inversion H.
       subst.
-      assert (eval C st e1 m = Resolved (EVal v1) (ST mem1 t1)) as RR1.
+      assert (eval C st e1 (Config C st (m_lete x e1 e2) :: l) m = Resolved (EVal v1) (ST mem1 t1) reached) as RR1.
       apply IHFUEL; eauto. nia.
       assert (eval (C [|dy_c_lete x t1 ([||])|]) 
                    (ST (t1 !-> v1; mem1) (update C (ST mem1 t1) x v1))
-                   e2 m = Resolved (MVal mv) st') as RR2.
+                   e2 reached m = Resolved (MVal mv) st' l') as RR2.
       apply IHFUEL; eauto. nia.
       simpl. rewrite RR1. rewrite RR2. eauto.
-    + remember (eval C st e1 FUEL) as v1.
+    + remember (eval C st e1 (Config C st (m_letm M e1 e2) :: l) FUEL) as v1.
       destruct v1 as [ | | v1 st1]; inversion H.
       clear H3. destruct v1 as [v1 | ]; inversion H.
       clear H3.
       remember (eval (C [|dy_c_letm M mv ([||])|]) st1
-                      e2 FUEL) as v2.
+                      e2 reached FUEL) as v2.
       destruct v2 as [ | | v2 st2]; inversion H.
       clear H3. destruct v2 as [v2 | ]; inversion H.
       subst.
-      assert (eval C st e1 m = Resolved (MVal mv) st1) as RR1.
+      assert (eval C st e1 (Config C st (m_letm M e1 e2) :: l) m = Resolved (MVal mv) st1 reached) as RR1.
       apply IHFUEL; eauto. nia.
       assert (eval (C [|dy_c_letm M mv ([||])|]) st1
-                   e2 m = Resolved (MVal mv0) st') as RR2.
+                   e2 reached m = Resolved (MVal mv0) st' l') as RR2.
       apply IHFUEL; eauto. nia.
       simpl. rewrite RR1. rewrite RR2. eauto.
 Qed.
       
 Lemma EvalR_well_defined_l :
-  forall `{time T} (C : @dy_ctx T) st e v st' (R : EvalR C st e v st'),
-    exists FUEL, eval C st e FUEL = Resolved v st'.
+  forall `{time T} (C : @dy_ctx T) st e l v st' (R : EvalR C st e v st'),
+    exists FUEL, 
+      match eval C st e l FUEL with
+      | Resolved v' st'' _ => v = v' /\ st' = st''
+      | _ => False
+      end.
 Proof.
-  intros. induction R.
+  intros. revert l. induction R; intros.
   - exists 1; simpl. rewrite <- ADDR. rewrite <- STATE. rewrite <- ACCESS. eauto.
   - exists 1; simpl; eauto.
-  - destruct IHR1 as [FUEL' EQ'].
-    destruct IHR2 as [FUEL'' EQ''].
-    destruct IHR3 as [FUEL''' EQ'''].
+  - destruct (IHR1 (Config C st (e_app e1 e2) :: l)) as [FUEL' EQ']. clear IHR1.
+    destruct (eval C st e1 (Config C st (e_app e1 e2) :: l) FUEL') eqn:EVAL1; try (inversion EQ'; fail).
+    destruct (IHR2 reached) as [FUEL'' EQ'']. clear IHR2.
+    destruct (eval C st_lam e2 reached FUEL'') eqn:EVAL2; try (inversion EQ''; fail).
+    destruct (IHR3 reached0) as [FUEL''' EQ''']. clear IHR3.
+    destruct (eval (C_lam [|dy_c_lam x t ([||])|])
+                   (ST (t !-> arg; mem) (update C (ST mem t) x arg)) e reached0
+                   FUEL''') eqn:EVAL3; try (inversion EQ'''; fail).
     exists (S (Nat.max FUEL' (Nat.max FUEL'' FUEL'''))).
     simpl.
-    assert (eval C st e1 (Nat.max FUEL' (Nat.max FUEL'' FUEL'''))
-            = Resolved (EVal (Closure x e C_lam)) st_lam) as RR.
+    destruct EQ' as [RR RR']. rewrite <- RR in *. rewrite <- RR' in *. clear RR RR'.
+    destruct EQ'' as [RR RR']. rewrite <- RR in *. rewrite <- RR' in *. clear RR RR'.
+    destruct EQ''' as [RR RR']. rewrite <- RR in *. rewrite <- RR' in *. clear RR RR'.
+    assert (eval C st e1 (Config C st (e_app e1 e2) :: l) (Nat.max FUEL' (Nat.max FUEL'' FUEL'''))
+            = Resolved (EVal (Closure x e C_lam)) st_lam reached) as RR.
     apply relax_fuel with (FUEL := FUEL'). nia. eauto.
     rewrite RR; clear RR.
-    assert (eval C st_lam e2 (Nat.max FUEL' (Nat.max FUEL'' FUEL'''))
-            = Resolved (EVal arg) (ST mem t)) as RR.
+    assert (eval C st_lam e2 reached (Nat.max FUEL' (Nat.max FUEL'' FUEL'''))
+            = Resolved (EVal arg) (ST mem t) reached0) as RR.
     apply relax_fuel with (FUEL := FUEL''). nia. eauto.
     rewrite RR; clear RR.
     assert (eval (C_lam [|dy_c_lam x t ([||])|]) 
-                 (ST (t !-> arg; mem) (update C (ST mem t) x arg)) e
+                 (ST (t !-> arg; mem) (update C (ST mem t) x arg)) e reached0
                  (Nat.max FUEL' (Nat.max FUEL'' FUEL'''))
-            = Resolved (EVal v) st_v) as RR.
+            = Resolved (EVal v) st_v reached1) as RR.
     apply relax_fuel with (FUEL := FUEL'''). nia. eauto.
     rewrite RR; clear RR. eauto.
-  - destruct IHR1 as [FUEL' EQ'].
-    destruct IHR2 as [FUEL'' EQ''].
+  - destruct (IHR1 (Config C st (e_link m e) :: l)) as [FUEL' EQ']. clear IHR1.
+    destruct (eval C st m (Config C st (e_link m e) :: l) FUEL') eqn:EVAL1; try (inversion EQ'; fail).
+    destruct (IHR2 reached) as [FUEL'' EQ'']. clear IHR2.
+    destruct (eval C_m st_m e reached FUEL'') eqn:EVAL2; try (inversion EQ''; fail).
     exists (S (Nat.max FUEL' FUEL'')).
     simpl.
-    assert (eval C st m (Nat.max FUEL' FUEL'')
-            = Resolved (MVal C_m) st_m) as RR.
+    destruct EQ' as [RR RR']. rewrite <- RR in *. rewrite <- RR' in *. clear RR RR'.
+    destruct EQ'' as [RR RR']. rewrite <- RR in *. rewrite <- RR' in *. clear RR RR'.
+    assert (eval C st m (Config C st (e_link m e) :: l) (Nat.max FUEL' FUEL'')
+            = Resolved (MVal C_m) st_m reached) as RR.
     apply relax_fuel with (FUEL := FUEL'). nia. eauto.
     rewrite RR; clear RR.
-    assert (eval C_m st_m e (Nat.max FUEL' FUEL'')
-            = Resolved v st_v) as RR.
+    assert (eval C_m st_m e reached (Nat.max FUEL' FUEL'')
+            = Resolved v st_v reached0) as RR.
     apply relax_fuel with (FUEL := FUEL''). nia. eauto.
     rewrite RR; clear RR. eauto. 
   - exists 1. simpl; eauto. 
   - exists 1; simpl. rewrite <- ACCESS. eauto. 
-  - destruct IHR1 as [FUEL' EQ'].
-    destruct IHR2 as [FUEL'' EQ''].
+  - destruct (IHR1 (Config C st (m_lete x e m) :: l)) as [FUEL' EQ']. clear IHR1.
+    destruct (eval C st e (Config C st (m_lete x e m) :: l) FUEL') eqn:EVAL1; try (inversion EQ'; fail).
+    destruct (IHR2 reached) as [FUEL'' EQ'']. clear IHR2.
+    destruct (eval (C [|dy_c_lete x t ([||])|])
+                   (ST (t !-> v; mem) (update C (ST mem t) x v)) m reached
+                   FUEL'') eqn:EVAL2; try (inversion EQ''; fail).
     exists (S (Nat.max FUEL' FUEL'')).
     simpl.
-    assert (eval C st e (Nat.max FUEL' FUEL'')
-            = Resolved (EVal v) (ST mem t)) as RR.
+    destruct EQ' as [RR RR']. rewrite <- RR in *. rewrite <- RR' in *. clear RR RR'.
+    destruct EQ'' as [RR RR']. rewrite <- RR in *. rewrite <- RR' in *. clear RR RR'.
+    assert (eval C st e (Config C st (m_lete x e m) :: l) (Nat.max FUEL' FUEL'')
+            = Resolved (EVal v) (ST mem t) reached) as RR.
     apply relax_fuel with (FUEL := FUEL'). nia. eauto.
     rewrite RR; clear RR.
     assert (eval (C [|dy_c_lete x t ([||])|]) 
-                 (ST (t !-> v; mem) (update C (ST mem t) x v)) m
+                 (ST (t !-> v; mem) (update C (ST mem t) x v)) m reached
                  (Nat.max FUEL' FUEL'')
-            = Resolved (MVal C_m) st_m) as RR.
+            = Resolved (MVal C_m) st_m reached0) as RR.
     apply relax_fuel with (FUEL := FUEL''). nia. eauto.
     rewrite RR; clear RR. eauto.
-  - destruct IHR1 as [FUEL' EQ'].
-    destruct IHR2 as [FUEL'' EQ''].
+  - destruct (IHR1 (Config C st (m_letm M m' m'') :: l)) as [FUEL' EQ']. clear IHR1.
+    destruct (eval C st m' (Config C st (m_letm M m' m'') :: l) FUEL') eqn:EVAL1; try (inversion EQ'; fail).
+    destruct (IHR2 reached) as [FUEL'' EQ'']. clear IHR2.
+    destruct (eval (C [|dy_c_letm M C' ([||])|]) st' m'' reached FUEL'') eqn:EVAL2; try (inversion EQ''; fail).
     exists (S (Nat.max FUEL' FUEL'')).
     simpl.
-    assert (eval C st m' (Nat.max FUEL' FUEL'')
-            = Resolved (MVal C') st') as RR.
+    destruct EQ' as [RR RR']. rewrite <- RR in *. rewrite <- RR' in *. clear RR RR'.
+    destruct EQ'' as [RR RR']. rewrite <- RR in *. rewrite <- RR' in *. clear RR RR'.
+    assert (eval C st m' (Config C st (m_letm M m' m'') :: l) (Nat.max FUEL' FUEL'')
+            = Resolved (MVal C') st' reached) as RR.
     apply relax_fuel with (FUEL := FUEL'). nia. eauto.
     rewrite RR; clear RR.
-    assert (eval (C [|dy_c_letm M C' ([||])|]) st' m'' (Nat.max FUEL' FUEL'')
-            = Resolved (MVal C'') st'') as RR.
+    assert (eval (C [|dy_c_letm M C' ([||])|]) st' m'' reached (Nat.max FUEL' FUEL'')
+            = Resolved (MVal C'') st'' reached0) as RR.
     apply relax_fuel with (FUEL := FUEL''). nia. eauto.
     rewrite RR; clear RR. eauto.
 Qed.
 
 Lemma EvalR_well_defined_r :
-  forall `{TIME : time T} FUEL (C : @dy_ctx T) st e v st' (R : eval C st e FUEL = Resolved v st'),
+  forall `{TIME : time T} FUEL (C : @dy_ctx T) st e l v st'
+    (R : match eval C st e l FUEL with
+         | Resolved v' st'' _ => v = v' /\ st' = st''
+         | _ => False
+         end),
     EvalR C st e v st'.
 Proof.
   intros. rename H into H'. rename H0 into H''. generalize dependent T. revert e.
   induction FUEL; intros; simpl in *; try (inversion R; fail).
   destruct e.
-  - remember (addr_x C x) as addr. destruct addr; inversion R. clear H0.
-    destruct st.
-    remember (mem t) as access.
-    destruct access; inversion R. subst. eauto.
-  - inversion R. eauto.
-  - remember (eval C st e1 FUEL) as v1.
-    destruct v1 as [ | | v1 st1]; inversion R.
-    clear H0. destruct v1 as [v1 | ]; inversion R.
-    clear H0. destruct v1 as [x v1 C_lam].
-    remember (eval C st1 e2 FUEL) as v2.
-    destruct v2 as [ | | v2 st2]; inversion R.
-    clear H0. destruct v2 as [v2 | ]; inversion R.
-    clear H0. destruct st2 as [mem2 t2].
+  - destruct (addr_x C x) eqn:ADDR;
+    destruct st; destruct (mem t) eqn:ACCESS; 
+    inversion R. subst. eauto.
+  - inversion R. subst. eauto.
+  - remember (eval C st e1 (Config C st (e_app e1 e2) :: l) FUEL) as v1.
+    destruct v1 as [ | | v1 st1]; try inversion R.
+    destruct v1 as [v1 | ]; try inversion R.
+    destruct v1 as [x v1 C_lam].
+    remember (eval C st1 e2 reached FUEL) as v2.
+    destruct v2 as [ | | v2 st2]; try inversion R.
+    destruct v2 as [v2 | ]; try inversion R.
+    destruct st2 as [mem2 t2].
     remember (eval (C_lam [|dy_c_lam x t2 ([||])|])
                    (ST (t2 !-> v2; mem2) (update C (ST mem2 t2) x v2)) 
-                   v1 FUEL) as v3.
-    destruct v3 as [ | | v3 st3]; inversion R.
-    clear H0. destruct v3 as [v3 | ]; inversion R.
+                   v1 reached0 FUEL) as v3.
+    destruct v3 as [ | | v3 st3]; try inversion R.
+    destruct v3 as [v3 | ]; try inversion R.
     subst.
-    assert (EvalR C st e1 (EVal (Closure x v1 C_lam)) st1) as RR1. eauto.
-    assert (EvalR C st1 e2 (EVal v2) (ST mem2 t2)) as RR2. eauto.
+    assert (EvalR C st e1 (EVal (Closure x v1 C_lam)) st1) as RR1. 
+    eapply IHFUEL; rewrite <- Heqv1; eauto.
+    assert (EvalR C st1 e2 (EVal v2) (ST mem2 t2)) as RR2.
+    eapply IHFUEL; rewrite <- Heqv2; eauto.
     assert (EvalR (C_lam [|dy_c_lam x t2 ([||])|])
                   (ST (t2 !-> v2; mem2) (update C (ST mem2 t2) x v2)) v1
-            (EVal v3) st') as RR3. eauto. eauto.
-  - remember (eval C st e1 FUEL) as v1.
-    destruct v1 as [ | | v1 st1]; inversion R.
-    clear H0. destruct v1 as [v1 | ]; inversion R.
-    clear H0. remember (eval mv st1 e2 FUEL) as v2.
+            (EVal v3) st3) as RR3. 
+    eapply IHFUEL; rewrite <- Heqv3; eauto. eauto.
+  - remember (eval C st e1 (Config C st (e_link e1 e2) :: l) FUEL) as v1.
+    destruct v1 as [ | | v1 st1]; try inversion R.
+    destruct v1 as [v1 | ]; try inversion R.
+    remember (eval mv st1 e2 reached FUEL) as v2.
     destruct v2 as [ | | v2 st2]; inversion R.
-    clear H0. destruct v2 as [v2 | ]; inversion R; subst;
-    eapply Eval_link; eauto.
+    assert (EvalR C st e1 (MVal mv) st1).
+    eapply IHFUEL; rewrite <- Heqv1; eauto.
+    assert (EvalR mv st1 e2 v2 st2).
+    eapply IHFUEL; rewrite <- Heqv2; eauto.
+    subst. eauto.
   - inversion R; subst. eapply Eval_empty; eauto.
   - remember (ctx_M C M) as ACCESS.
     destruct ACCESS; inversion R; subst. eapply Eval_var_m; eauto.
-  - remember (eval C st e1 FUEL) as v1.
-    destruct v1 as [ | | v1 st1]; inversion R.
-    clear H0. destruct v1 as [v1 | ]; inversion R.
-    clear H0. destruct st1 as [mem1 t1].
+  - remember (eval C st e1 (Config C st (m_lete x e1 e2) :: l) FUEL) as v1.
+    destruct v1 as [ | | v1 st1]; try inversion R.
+    destruct v1 as [v1 | ]; try inversion R.
+    destruct st1 as [mem1 t1].
     remember (eval (C [|dy_c_lete x t1 ([||])|])
                    (ST (t1 !-> v1; mem1) (update C (ST mem1 t1) x v1)) 
-                   e2 FUEL) as v2.
-    destruct v2 as [ | | v2 st2]; inversion R.
-    clear H0. destruct v2 as [v2 | ]; inversion R.
-    subst.
-    assert (EvalR C st e1 (EVal v1) (ST mem1 t1)) as RR1. eauto.
+                   e2 reached FUEL) as v2.
+    destruct v2 as [ | | v2 st2]; try inversion R.
+    destruct v2 as [v2 | ]; inversion R.
+    assert (EvalR C st e1 (EVal v1) (ST mem1 t1)).
+    eapply IHFUEL; rewrite <- Heqv1; eauto.
     assert (EvalR (C [|dy_c_lete x t1 ([||])|])
                   (ST (t1 !-> v1; mem1) (update C (ST mem1 t1) x v1)) e2
-            (MVal mv) st') as RR2. eauto.
-    eapply Eval_lete; eauto.
-  - remember (eval C st e1 FUEL) as v1.
-    destruct v1 as [ | | v1 st1]; inversion R.
-    clear H0. destruct v1 as [v1 | ]; inversion R.
-    clear H0.
-    remember (eval (C [|dy_c_letm M mv ([||])|]) st1 e2 FUEL) as v2.
-    destruct v2 as [ | | v2 st2]; inversion R.
-    clear H0. destruct v2 as [v2 | ]; inversion R.
-    subst.
-    assert (EvalR C st e1 (MVal mv) st1) as RR1. eauto.
-    assert (EvalR (C [|dy_c_letm M mv ([||])|])
-                  st1 e2 (MVal mv0) st') as RR2. eauto.
-    eapply Eval_letm; eauto.
+            (MVal mv) st2).
+    eapply IHFUEL; rewrite <- Heqv2; eauto.
+    subst. eauto.
+  - remember (eval C st e1 (Config C st (m_letm M e1 e2) :: l) FUEL) as v1.
+    destruct v1 as [ | | v1 st1]; try inversion R.
+    destruct v1 as [v1 | ]; try inversion R.
+    remember (eval (C [|dy_c_letm M mv ([||])|]) st1 e2 reached FUEL) as v2.
+    destruct v2 as [ | | v2 st2]; try inversion R.
+    destruct v2 as [v2 | ]; inversion R.
+    assert (EvalR C st e1 (MVal mv) st1).
+    eapply IHFUEL; rewrite <- Heqv1; eauto.
+    assert (EvalR (C [|dy_c_letm M mv ([||])|]) st1 e2 (MVal mv0) st2).
+    eapply IHFUEL; rewrite <- Heqv2; eauto.
+    subst. eauto.
 Qed.
 
 Theorem EvalR_well_defined :
-  forall `{TIME : time T} C st e v st',
-    (exists FUEL, eval C st e FUEL = Resolved v st') <->
+  forall `{TIME : time T} l C st e v st',
+    (exists FUEL, 
+      match eval C st e l FUEL with 
+      | Resolved v' st'' _ => v = v' /\ st' = st''
+      | _ => False
+      end) <->
     EvalR C st e v st'.
 Proof.
   intros; split; try apply EvalR_well_defined_l.
@@ -479,6 +523,1095 @@ Proof.
   revert C3 st3.
   induction REACH1; eauto.
 Qed.
+
+Definition extract_reached {T} (interp : @interpreter_state T) :=
+  match interp with
+  | Pending reached
+  | Error reached
+  | Resolved _ _ reached => reached
+  end.
+
+Lemma reach_myself :
+  forall `{TIME : time T} (C : @dy_ctx T) st e l FUEL,
+    In (Config C st e) (extract_reached (eval C st e l FUEL)) /\
+    (forall cf, In cf l -> In cf (extract_reached (eval C st e l FUEL))).
+Proof.
+  intros. rename H into H'. rename H0 into H''.
+  revert C st e l; induction FUEL; intros; try (simpl; eauto; fail).
+  split.
+  - simpl. destruct e.
+    + destruct (addr_x C x) as [addr | ]; try destruct st;
+      try destruct (mem addr); simpl; eauto.
+    + simpl; eauto.
+    + specialize (IHFUEL C st e1 (Config C st (e_app e1 e2) :: l)) as IH.
+      destruct IH as [IH IH'].
+      destruct (eval C st e1 (Config C st (e_app e1 e2) :: l) FUEL);
+      assert (In (Config C st (e_app e1 e2)) reached); try apply IH'; simpl; eauto.
+      destruct v; simpl; eauto.
+      destruct ev as [x e C']. clear IH IH'.
+      specialize (IHFUEL C st0 e2 reached) as IH.
+      destruct IH as [IH IH'].
+      destruct (eval C st0 e2 reached FUEL); eauto.
+      destruct v; eauto. destruct st1.
+      assert (In (Config C st (e_app e1 e2)) reached0); eauto. clear IH IH'.
+      specialize (IHFUEL (C' [|dy_c_lam x t ([||])|]) (ST (t !-> ev; mem) (update C (ST mem t) x ev)) e reached0) as IH.
+      destruct IH as [IH IH'].
+      destruct (eval (C' [|dy_c_lam x t ([||])|])
+                (ST (t !-> ev; mem) (update C (ST mem t) x ev)) e reached0
+                FUEL); eauto.
+      destruct v; eauto.
+    + specialize (IHFUEL C st e1 (Config C st (e_link e1 e2) :: l)) as IH.
+      destruct IH as [IH IH'].
+      destruct (eval C st e1 (Config C st (e_link e1 e2) :: l) FUEL);
+      assert (In (Config C st (e_link e1 e2)) reached); try apply IH'; simpl; eauto.
+      destruct v; simpl; eauto. clear IH IH'.
+      specialize (IHFUEL mv st0 e2 reached) as IH.
+      destruct IH as [IH IH'].
+      destruct (eval mv st0 e2 reached FUEL); eauto.
+    + simpl. eauto.
+    + destruct (ctx_M C M); simpl; eauto.
+    + specialize (IHFUEL C st e1 (Config C st (m_lete x e1 e2) :: l)) as IH.
+      destruct IH as [IH IH'].
+      destruct (eval C st e1 (Config C st (m_lete x e1 e2) :: l) FUEL);
+      assert (In (Config C st (m_lete x e1 e2)) reached); try apply IH'; simpl; eauto.
+      destruct v; simpl; eauto. destruct st0. clear IH IH'.
+      specialize (IHFUEL (C [|dy_c_lete x t ([||])|]) (ST (t !-> ev; mem) (update C (ST mem t) x ev)) e2 reached) as IH.
+      destruct IH as [IH IH'].
+      destruct (eval (C [|dy_c_lete x t ([||])|])
+                     (ST (t !-> ev; mem) (update C (ST mem t) x ev)) e2 reached
+                     FUEL); eauto.
+      destruct v; eauto.
+    + specialize (IHFUEL C st e1 (Config C st (m_letm M e1 e2) :: l)) as IH.
+      destruct IH as [IH IH'].
+      destruct (eval C st e1 (Config C st (m_letm M e1 e2) :: l) FUEL);
+      assert (In (Config C st (m_letm M e1 e2)) reached); try apply IH'; simpl; eauto.
+      destruct v; simpl; eauto. clear IH IH'.
+      specialize (IHFUEL (C [|dy_c_letm M mv ([||])|]) st0 e2 reached) as IH.
+      destruct IH as [IH IH'].
+      destruct (eval (C [|dy_c_letm M mv ([||])|]) st0 e2 reached FUEL); eauto.
+      destruct v; eauto.
+  - intros. destruct e; simpl; eauto.
+    + destruct (addr_x C x); simpl; eauto. destruct st. destruct (mem t); simpl; eauto.
+    + specialize (IHFUEL C st e1 (Config C st (e_app e1 e2) :: l)) as IH.
+      destruct IH as [IH IH'].
+      destruct (eval C st e1 (Config C st (e_app e1 e2) :: l) FUEL);
+      assert (In cf reached); simpl in *; eauto.
+      destruct v; simpl; eauto.
+      destruct ev as [x e C']. clear IH IH'.
+      specialize (IHFUEL C st0 e2 reached) as IH.
+      destruct IH as [IH IH'].
+      destruct (eval C st0 e2 reached FUEL); eauto.
+      destruct v; eauto. destruct st1.
+      assert (In cf reached0); simpl in *; eauto. clear IH IH'.
+      specialize (IHFUEL (C' [|dy_c_lam x t ([||])|]) (ST (t !-> ev; mem) (update C (ST mem t) x ev)) e reached0) as IH.
+      destruct IH as [IH IH'].
+      destruct (eval (C' [|dy_c_lam x t ([||])|])
+                (ST (t !-> ev; mem) (update C (ST mem t) x ev)) e reached0
+                FUEL); eauto.
+      destruct v; eauto.
+    + specialize (IHFUEL C st e1 (Config C st (e_link e1 e2) :: l)) as IH.
+      destruct IH as [IH IH'].
+      destruct (eval C st e1 (Config C st (e_link e1 e2) :: l) FUEL);
+      assert (In cf reached); try apply IH'; simpl; eauto.
+      destruct v; simpl; eauto. clear IH IH'.
+      specialize (IHFUEL mv st0 e2 reached) as IH.
+      destruct IH as [IH IH'].
+      destruct (eval mv st0 e2 reached FUEL); eauto.
+    + destruct (ctx_M C M); simpl; eauto.
+    + specialize (IHFUEL C st e1 (Config C st (m_lete x e1 e2) :: l)) as IH.
+      destruct IH as [IH IH'].
+      destruct (eval C st e1 (Config C st (m_lete x e1 e2) :: l) FUEL);
+      assert (In cf reached); try apply IH'; simpl; eauto.
+      destruct v; simpl; eauto. destruct st0. clear IH IH'.
+      specialize (IHFUEL (C [|dy_c_lete x t ([||])|]) (ST (t !-> ev; mem) (update C (ST mem t) x ev)) e2 reached) as IH.
+      destruct IH as [IH IH'].
+      destruct (eval (C [|dy_c_lete x t ([||])|])
+                     (ST (t !-> ev; mem) (update C (ST mem t) x ev)) e2 reached
+                     FUEL); eauto.
+      destruct v; eauto.
+    + specialize (IHFUEL C st e1 (Config C st (m_letm M e1 e2) :: l)) as IH.
+      destruct IH as [IH IH'].
+      destruct (eval C st e1 (Config C st (m_letm M e1 e2) :: l) FUEL);
+      assert (In cf reached); try apply IH'; simpl; eauto.
+      destruct v; simpl; eauto. clear IH IH'.
+      specialize (IHFUEL (C [|dy_c_letm M mv ([||])|]) st0 e2 reached) as IH.
+      destruct IH as [IH IH'].
+      destruct (eval (C [|dy_c_letm M mv ([||])|]) st0 e2 reached FUEL); eauto.
+      destruct v; eauto.
+Qed.
+
+Lemma relax_fuel_reach :
+  forall `{TIME : time T} (C : @dy_ctx T) st e l cf FUEL FUEL' (LE : FUEL <= FUEL'),
+    In cf (extract_reached (eval C st e l FUEL)) ->
+    In cf (extract_reached (eval C st e l FUEL')).
+Proof.
+  intros. rename H into H'. rename H0 into H''. rename H1 into H.
+  revert C st e l FUEL' LE H.
+  induction FUEL; intros.
+  - pose proof (reach_myself C st e l FUEL') as [HINT HINT'].
+    inversion H; eauto. rewrite <- H0; eauto.
+  - simpl in H; destruct e; inversion LE; eauto; assert (FUEL <= m) as LE'; try nia.
+    + specialize (IHFUEL C st e1 (Config C st (e_app e1 e2) :: l) m LE') as HINT.
+      destruct (eval C st e1 (Config C st (e_app e1 e2) :: l) FUEL) eqn:EVAL1; simpl;
+      destruct (eval C st e1 (Config C st (e_app e1 e2) :: l) m) eqn:EVAL1'; eauto;
+      try (
+        assert (In cf (extract_reached (eval C st0 e2 reached0 m))) as HINT';
+        try (apply reach_myself; apply HINT; eauto);
+        destruct v; eauto; destruct ev;
+        destruct (eval C st0 e2 reached0 m); eauto;
+        destruct v; eauto; destruct st1;
+        assert (In cf (extract_reached (eval (C0 [|dy_c_lam x t ([||])|])
+                                             (ST (t !-> ev; mem) (update C (ST mem t) x ev)) e
+                                             reached1 m))) as HINT'';
+        try (apply reach_myself; apply HINT');
+        destruct (eval (C0 [|dy_c_lam x t ([||])|])
+                       (ST (t !-> ev; mem) (update C (ST mem t) x ev)) e
+                       reached1 m); eauto; destruct v; eauto; fail);
+      pose proof (relax_fuel C st e1 (Config C st (e_app e1 e2) :: l) reached v st0 FUEL m LE' EVAL1) as RR;
+      rewrite RR in EVAL1'; inversion EVAL1'; subst.
+      destruct v0; eauto. destruct ev.
+      specialize (IHFUEL C st1 e2 reached0 m LE') as HINT'.
+      destruct (eval C st1 e2 reached0 FUEL) eqn:EVAL2;
+      destruct (eval C st1 e2 reached0 m) eqn:EVAL2'; eauto;
+      try (
+        specialize (HINT' H); destruct v; eauto; destruct st0;
+        assert (In cf (extract_reached (eval (C0 [|dy_c_lam x t ([||])|])
+                                           (ST (t !-> ev; mem) (update C (ST mem t) x ev)) e
+                                           reached1 m))) as HINT'';
+        try (apply reach_myself; apply HINT');
+        destruct (eval (C0 [|dy_c_lam x t ([||])|])
+                       (ST (t !-> ev; mem) (update C (ST mem t) x ev)) e
+                       reached1 m); eauto; destruct v; eauto);
+      pose proof (relax_fuel C st1 e2 reached0 reached v st0 FUEL m LE' EVAL2) as RR';
+      rewrite RR' in EVAL2'; inversion EVAL2'; subst.
+      destruct v0; eauto. destruct st2.
+      specialize (IHFUEL (C0 [|dy_c_lam x t ([||])|])
+                         (ST (t !-> ev; mem) (update C (ST mem t) x ev)) e
+                         reached1 m LE') as HINT''.
+      destruct (eval (C0 [|dy_c_lam x t ([||])|])
+                     (ST (t !-> ev; mem) (update C (ST mem t) x ev)) e
+                     reached1 FUEL) eqn:EVAL3;
+      destruct (eval (C0 [|dy_c_lam x t ([||])|])
+                     (ST (t !-> ev; mem) (update C (ST mem t) x ev)) e
+                     reached1 m) eqn:EVAL3'; eauto;
+      try (destruct v; eauto); destruct v0; eauto.
+    + specialize (IHFUEL C st e1 (Config C st (e_link e1 e2) :: l) m LE') as HINT.
+      destruct (eval C st e1 (Config C st (e_link e1 e2) :: l) FUEL) eqn:EVAL1; simpl;
+      destruct (eval C st e1 (Config C st (e_link e1 e2) :: l) m) eqn:EVAL1'; eauto;
+      try (
+        destruct v; eauto;
+        assert (In cf (extract_reached (eval mv st0 e2 reached0 m))) as HINT';
+        try (apply reach_myself; apply HINT; eauto);
+        destruct (eval mv st0 e2 reached0 m); eauto; fail);
+      pose proof (relax_fuel C st e1 (Config C st (e_link e1 e2) :: l) reached v st0 FUEL m LE' EVAL1) as RR;
+      rewrite RR in EVAL1'; inversion EVAL1'; subst.
+      destruct v0; eauto.
+      destruct (eval mv st1 e2 reached0 FUEL) eqn:EVAL2; simpl;
+      destruct (eval mv st1 e2 reached0 m) eqn:EVAL2';
+      try (
+        assert (In cf (extract_reached (eval mv st1 e2 reached0 m))) as HINT';
+        try (apply IHFUEL; eauto; rewrite EVAL2; eauto);
+        rewrite EVAL2' in HINT'; eauto).
+    + specialize (IHFUEL C st e1 (Config C st (m_lete x e1 e2) :: l) m LE') as HINT.
+      destruct (eval C st e1 (Config C st (m_lete x e1 e2) :: l) FUEL) eqn:EVAL1; simpl;
+      destruct (eval C st e1 (Config C st (m_lete x e1 e2) :: l) m) eqn:EVAL1'; eauto;
+      try (
+        destruct v; eauto; destruct st0;
+        assert (In cf (extract_reached (eval (C [|dy_c_lete x t ([||])|])
+                                             (ST (t !-> ev; mem) (update C (ST mem t) x ev)) e2
+                                             reached0 m))) as HINT';
+        try (apply reach_myself; apply HINT; eauto);
+        destruct (eval (C [|dy_c_lete x t ([||])|])
+                       (ST (t !-> ev; mem) (update C (ST mem t) x ev)) e2
+                       reached0 m); eauto; destruct v; eauto; fail);
+      pose proof (relax_fuel C st e1 (Config C st (m_lete x e1 e2) :: l) reached v st0 FUEL m LE' EVAL1) as RR;
+      rewrite RR in EVAL1'; inversion EVAL1'; subst.
+      destruct v0; eauto. destruct st1.
+      destruct (eval (C [|dy_c_lete x t ([||])|])
+                     (ST (t !-> ev; mem) (update C (ST mem t) x ev)) e2 reached0
+                     FUEL) eqn:EVAL2; simpl;
+      destruct (eval (C [|dy_c_lete x t ([||])|])
+                     (ST (t !-> ev; mem) (update C (ST mem t) x ev)) e2 reached0
+                     m) eqn:EVAL2';
+      try (
+        assert (In cf (extract_reached (eval (C [|dy_c_lete x t ([||])|])
+                                             (ST (t !-> ev; mem) (update C (ST mem t) x ev)) e2 reached0
+                                             m))) as HINT';
+        try (apply IHFUEL; eauto; rewrite EVAL2; eauto);
+        rewrite EVAL2' in HINT'; eauto; destruct v; eauto);
+      pose proof (relax_fuel (C [|dy_c_lete x t ([||])|])
+                             (ST (t !-> ev; mem) (update C (ST mem t) x ev)) e2
+                             reached0 reached v st0 FUEL m LE' EVAL2) as RR';
+      rewrite RR' in EVAL2'; inversion EVAL2'; subst.
+      destruct v0; eauto.
+    + specialize (IHFUEL C st e1 (Config C st (m_letm M e1 e2) :: l) m LE') as HINT.
+      destruct (eval C st e1 (Config C st (m_letm M e1 e2) :: l) FUEL) eqn:EVAL1; simpl;
+      destruct (eval C st e1 (Config C st (m_letm M e1 e2) :: l) m) eqn:EVAL1'; eauto;
+      try (
+        destruct v; eauto;
+        assert (In cf (extract_reached (eval (C [|dy_c_letm M mv ([||])|]) st0 e2 reached0 m))) as HINT';
+        try (apply reach_myself; apply HINT; eauto);
+        destruct (eval (C [|dy_c_letm M mv ([||])|]) st0 e2 reached0 m); eauto; destruct v; eauto; fail);
+      pose proof (relax_fuel C st e1 (Config C st (m_letm M e1 e2) :: l) reached v st0 FUEL m LE' EVAL1) as RR;
+      rewrite RR in EVAL1'; inversion EVAL1'; subst.
+      destruct v0; eauto.
+      destruct (eval (C [|dy_c_letm M mv ([||])|]) st1 e2 reached0 FUEL) eqn:EVAL2; simpl;
+      destruct (eval (C [|dy_c_letm M mv ([||])|]) st1 e2 reached0 m) eqn:EVAL2';
+      try (
+        assert (In cf (extract_reached (eval (C [|dy_c_letm M mv ([||])|]) st1 e2 reached0 m))) as HINT';
+        try (apply IHFUEL; eauto; rewrite EVAL2; eauto);
+        rewrite EVAL2' in HINT'; eauto; destruct v; eauto; fail);
+      pose proof (relax_fuel (C [|dy_c_letm M mv ([||])|]) st1 e2 reached0 reached v st0 FUEL m LE' EVAL2) as RR';
+      rewrite RR' in EVAL2'; inversion EVAL2'; subst.
+      destruct v0; eauto.
+Qed.
+
+Lemma reach_same :
+  forall `{TIME : time T} FUEL (C : @dy_ctx T) st e l l'
+          (CONTAINED : forall cf, In cf l -> In cf l'),
+    match (eval C st e l FUEL), (eval C st e l' FUEL) with
+    | Resolved v st_v reached, Resolved v' st_v' reached' => 
+      v = v' /\ st_v = st_v' /\ (forall cf, In cf reached -> In cf reached')
+    | Error reached, Error reached'
+    | Pending reached, Pending reached' =>
+      forall cf, In cf reached -> In cf reached'
+    | _, _ => False
+    end.
+Proof.
+  intros. rename H into ET. rename H0 into OT.
+  revert C st e l l' CONTAINED. induction FUEL; intros.
+  simpl. intros. destruct H; eauto.
+  destruct e; simpl; eauto.
+  - destruct (addr_x C x); destruct st; destruct (mem t); repeat split; intros; destruct H; simpl; eauto.
+  - repeat split; intros; destruct H; eauto.
+  - assert ((forall cf : config,
+                    In cf (Config C st (e_app e1 e2) :: l) ->
+                    In cf (Config C st (e_app e1 e2) :: l'))) as CONTAINED'.
+    { intros. simpl in *. destruct H; eauto. }
+    specialize (IHFUEL C st e1 (Config C st (e_app e1 e2) :: l) (Config C st (e_app e1 e2) :: l') CONTAINED') as IHl.
+    clear CONTAINED'.
+    destruct (eval C st e1 (Config C st (e_app e1 e2) :: l) FUEL);
+    destruct (eval C st e1 (Config C st (e_app e1 e2) :: l') FUEL);
+    try (assert False as contra; eauto; inversion contra); eauto.
+    destruct IHl as [RR [RR' CONTAINED']]. rewrite <- RR in *. rewrite <- RR' in *. clear RR RR'.
+    destruct v; eauto. destruct ev.
+    specialize (IHFUEL C st0 e2 reached reached0 CONTAINED') as IHr.
+    clear CONTAINED'.
+    destruct (eval C st0 e2 reached FUEL);
+    destruct (eval C st0 e2 reached0 FUEL);
+    try (assert False as contra; eauto; inversion contra); eauto.
+    destruct IHr as [RR [RR' CONTAINED']]. rewrite <- RR in *. rewrite <- RR' in *. clear RR RR'.
+    destruct v; eauto. destruct st2.
+    specialize (IHFUEL (C0 [|dy_c_lam x t ([||])|])
+                       (ST (t !-> ev; mem) (update C (ST mem t) x ev))
+                       e reached1 reached2 CONTAINED').
+    clear CONTAINED'.
+    destruct (eval (C0 [|dy_c_lam x t ([||])|])
+                   (ST (t !-> ev; mem) (update C (ST mem t) x ev))
+                   e reached1 FUEL);
+    destruct (eval (C0 [|dy_c_lam x t ([||])|])
+                   (ST (t !-> ev; mem) (update C (ST mem t) x ev))
+                   e reached2 FUEL);
+    try (assert False as contra; eauto; inversion contra); eauto.
+    destruct IHFUEL as [RR [RR' CONTAINED']]. rewrite <- RR in *. rewrite <- RR' in *. clear RR RR'.
+    destruct v; eauto.
+  - assert ((forall cf : config,
+                    In cf (Config C st (e_link e1 e2) :: l) ->
+                    In cf (Config C st (e_link e1 e2) :: l'))) as CONTAINED'.
+    { intros. simpl in *. destruct H; eauto. }
+    specialize (IHFUEL C st e1 (Config C st (e_link e1 e2) :: l) (Config C st (e_link e1 e2) :: l') CONTAINED') as IHl.
+    clear CONTAINED'.
+    destruct (eval C st e1 (Config C st (e_link e1 e2) :: l) FUEL);
+    destruct (eval C st e1 (Config C st (e_link e1 e2) :: l') FUEL);
+    try (assert False as contra; eauto; inversion contra); eauto.
+    destruct IHl as [RR [RR' CONTAINED']]. rewrite <- RR in *. rewrite <- RR' in *. clear RR RR'.
+    destruct v; eauto.
+    specialize (IHFUEL mv st0 e2 reached reached0 CONTAINED') as IHr. clear CONTAINED'.
+    destruct (eval mv st0 e2 reached FUEL);
+    destruct (eval mv st0 e2 reached0 FUEL);
+    try (assert False as contra; eauto; inversion contra); eauto.
+  - repeat split; eauto. intros; destruct H; eauto.
+  - destruct (ctx_M C M); eauto; repeat split; intros; simpl in *; destruct H; eauto.
+  - assert ((forall cf : config,
+                    In cf (Config C st (m_lete x e1 e2) :: l) ->
+                    In cf (Config C st (m_lete x e1 e2) :: l'))) as CONTAINED'.
+    { intros. simpl in *. destruct H; eauto. }
+    specialize (IHFUEL C st e1 (Config C st (m_lete x e1 e2) :: l) (Config C st (m_lete x e1 e2) :: l') CONTAINED') as IHl.
+    clear CONTAINED'.
+    destruct (eval C st e1 (Config C st (m_lete x e1 e2) :: l) FUEL);
+    destruct (eval C st e1 (Config C st (m_lete x e1 e2) :: l') FUEL);
+    try (assert False as contra; eauto; inversion contra); eauto.
+    destruct IHl as [RR [RR' CONTAINED']]. rewrite <- RR in *. rewrite <- RR' in *. clear RR RR'.
+    destruct v; eauto. destruct st0.
+    specialize (IHFUEL (C [|dy_c_lete x t ([||])|])
+                       (ST (t !-> ev; mem) (update C (ST mem t) x ev))
+                       e2 reached reached0 CONTAINED'). clear CONTAINED'.
+    destruct (eval (C [|dy_c_lete x t ([||])|])
+                   (ST (t !-> ev; mem) (update C (ST mem t) x ev))
+                   e2 reached FUEL);
+    destruct (eval (C [|dy_c_lete x t ([||])|])
+                   (ST (t !-> ev; mem) (update C (ST mem t) x ev))
+                   e2 reached0 FUEL);
+    try (assert False as contra; eauto; inversion contra); eauto.
+    destruct IHFUEL as [RR [RR' CONTAINED']]. rewrite <- RR in *. rewrite <- RR' in *.
+    destruct v; eauto.
+  - assert ((forall cf : config,
+                    In cf (Config C st (m_letm M e1 e2) :: l) ->
+                    In cf (Config C st (m_letm M e1 e2) :: l'))) as CONTAINED'.
+    { intros. simpl in *. destruct H; eauto. }
+    specialize (IHFUEL C st e1 (Config C st (m_letm M e1 e2) :: l) (Config C st (m_letm M e1 e2) :: l') CONTAINED') as IHl.
+    clear CONTAINED'.
+    destruct (eval C st e1 (Config C st (m_letm M e1 e2) :: l) FUEL);
+    destruct (eval C st e1 (Config C st (m_letm M e1 e2) :: l') FUEL);
+    try (assert False as contra; eauto; inversion contra); eauto.
+    destruct IHl as [RR [RR' CONTAINED']]. rewrite <- RR in *. rewrite <- RR' in *. clear RR RR'.
+    destruct v; eauto.
+    specialize (IHFUEL (C [|dy_c_letm M mv ([||])|]) st0 e2 reached reached0 CONTAINED'). clear CONTAINED'.
+    destruct (eval (C [|dy_c_letm M mv ([||])|]) st0 e2 reached FUEL);
+    destruct (eval (C [|dy_c_letm M mv ([||])|]) st0 e2 reached0 FUEL);
+    try (assert False as contra; eauto; inversion contra); eauto.
+    destruct IHFUEL as [RR [RR' CONTAINED']]. rewrite <- RR in *. rewrite <- RR' in *.
+    destruct v; eauto.
+Qed.
+
+Lemma separate_reach :
+  forall `{TIME : time T} FUEL (C : @dy_ctx T) st e l cf,
+    In cf (extract_reached (eval C st e l FUEL)) <->
+    In cf l \/ In cf (extract_reached (eval C st e [] FUEL)).
+Proof.
+  intros. rename H into ET. rename H0 into OT.
+  revert C st e l cf. induction FUEL; intros; simpl; split; intros.
+  - destruct H; eauto. 
+  - destruct H as [?|[?|?]]; eauto. exfalso; eauto.
+  - destruct e.
+    + destruct (addr_x C x); destruct st; destruct (mem t); simpl in *;
+      destruct H; eauto.
+    + simpl in *; destruct H; eauto.
+    + specialize (IHFUEL C st e1 (Config C st (e_app e1 e2) :: l) cf) as HINT1.
+      specialize (IHFUEL C st e1 [Config C st (e_app e1 e2)] cf) as HINT1'.
+      assert (forall cf, In cf [Config C st (e_app e1 e2)] ->
+                         In cf (Config C st (e_app e1 e2) :: l)) as CONTAINED.
+      { intros; simpl in *; destruct H0; eauto. inversion H0. }
+      pose proof (reach_same FUEL C st e1 [Config C st (e_app e1 e2)] (Config C st (e_app e1 e2) :: l) CONTAINED) as contra.
+      clear CONTAINED.
+      destruct (eval C st e1 (Config C st (e_app e1 e2) :: l) FUEL);
+      destruct (eval C st e1 [Config C st (e_app e1 e2)] FUEL);
+      try (rewrite HINT1 in H); try rewrite HINT1';
+      try (simpl in *; destruct H as [[?|?]|?]; eauto; fail);
+      try (inversion contra; fail).
+      destruct contra as [RR [RR' CONTAINED]]. rewrite RR in *. rewrite RR' in *. clear RR RR'.
+      destruct v;
+      try (rewrite HINT1 in H; rewrite HINT1'; destruct H as [[?|?]|?]; simpl in *; eauto).
+      destruct ev. simpl in *.
+      specialize (IHFUEL C st0 e2 reached cf) as HINT2.
+      specialize (IHFUEL C st0 e2 reached0 cf) as HINT2'.
+      pose proof (reach_same FUEL C st0 e2 reached0 reached CONTAINED) as contra.
+      clear CONTAINED.
+      destruct (eval C st0 e2 reached FUEL);
+      destruct (eval C st0 e2 reached0 FUEL);
+      try (rewrite HINT2 in H); try rewrite HINT2';
+      try (rewrite HINT1 in H); try rewrite HINT1';
+      try (simpl in *; destruct H as [[[?|?]|?]|?]; eauto; fail);
+      try (inversion contra; fail).
+      destruct contra as [RR [RR' CONTAINED]]. rewrite RR in *. rewrite RR' in *. clear RR RR'.
+      destruct v;
+      try (rewrite HINT2 in H; rewrite HINT2'; rewrite HINT1 in H; rewrite HINT1';
+          destruct H as [[[?|?]|?]|?]; simpl in *; eauto).
+      destruct st2.
+      specialize (IHFUEL (C0 [|dy_c_lam x t ([||])|])
+                         (ST (t !-> ev; mem) (update C (ST mem t) x ev)) 
+                         e reached1 cf) as HINT3.
+      specialize (IHFUEL (C0 [|dy_c_lam x t ([||])|])
+                         (ST (t !-> ev; mem) (update C (ST mem t) x ev)) 
+                         e reached2 cf) as HINT3'.
+      pose proof (reach_same FUEL (C0 [|dy_c_lam x t ([||])|])
+                                  (ST (t !-> ev; mem) (update C (ST mem t) x ev))
+                                  e reached2 reached1 CONTAINED) as contra. clear CONTAINED.
+      destruct (eval (C0 [|dy_c_lam x t ([||])|])
+                     (ST (t !-> ev; mem) (update C (ST mem t) x ev)) e
+                     reached1 FUEL);
+      destruct (eval (C0 [|dy_c_lam x t ([||])|])
+                     (ST (t !-> ev; mem) (update C (ST mem t) x ev)) e
+                     reached2 FUEL);
+      try (rewrite HINT3 in H); try rewrite HINT3';
+      try (rewrite HINT2 in H); try rewrite HINT2';
+      try (rewrite HINT1 in H); try rewrite HINT1';
+      try (simpl in *; destruct H as [[[[?|?]|?]|?]|?]; eauto 7; fail);
+      try (inversion contra; fail).
+      destruct contra as [RR [RR' CONTAINED]]. rewrite RR in *. rewrite RR' in *. clear RR RR'.
+      destruct v; simpl in *;
+      rewrite HINT3 in H; rewrite HINT3';
+      rewrite HINT2 in H; rewrite HINT2';
+      rewrite HINT1 in H; rewrite HINT1';
+      destruct H as [[[[?|?]|?]|?]|?]; eauto 7.
+    + specialize (IHFUEL C st e1 (Config C st (e_link e1 e2) :: l) cf) as HINT1.
+      specialize (IHFUEL C st e1 [Config C st (e_link e1 e2)] cf) as HINT1'.
+      assert (forall cf, In cf [Config C st (e_link e1 e2)] ->
+                         In cf (Config C st (e_link e1 e2) :: l)) as CONTAINED.
+      { intros; simpl in *; destruct H0; eauto. inversion H0. }
+      pose proof (reach_same FUEL C st e1 [Config C st (e_link e1 e2)] (Config C st (e_link e1 e2) :: l) CONTAINED) as contra.
+      clear CONTAINED.
+      destruct (eval C st e1 (Config C st (e_link e1 e2) :: l) FUEL);
+      destruct (eval C st e1 [Config C st (e_link e1 e2)] FUEL);
+      try (rewrite HINT1 in H); try rewrite HINT1';
+      try (simpl in *; destruct H as [[?|?]|?]; eauto; fail);
+      try (inversion contra; fail).
+      destruct contra as [RR [RR' CONTAINED]]. rewrite RR in *. rewrite RR' in *. clear RR RR'.
+      destruct v;
+      try (rewrite HINT1 in H; rewrite HINT1'; destruct H as [[?|?]|?]; simpl in *; eauto).
+      specialize (IHFUEL mv st0 e2 reached cf) as HINT2.
+      specialize (IHFUEL mv st0 e2 reached0 cf) as HINT2'.
+      pose proof (reach_same FUEL mv st0 e2 reached0 reached CONTAINED) as contra.
+      clear CONTAINED.
+      destruct (eval mv st0 e2 reached FUEL);
+      destruct (eval mv st0 e2 reached0 FUEL);
+      try (rewrite HINT2 in H); try rewrite HINT2';
+      try (rewrite HINT1 in H); try rewrite HINT1';
+      try (simpl in *; destruct H as [[[?|?]|?]|?]; eauto; fail);
+      try (inversion contra; fail).
+    + simpl in *. destruct H; eauto.
+    + destruct (ctx_M C M); simpl in *; destruct H; eauto.
+    + specialize (IHFUEL C st e1 (Config C st (m_lete x e1 e2) :: l) cf) as HINT1.
+      specialize (IHFUEL C st e1 [Config C st (m_lete x e1 e2)] cf) as HINT1'.
+      assert (forall cf, In cf [Config C st (m_lete x e1 e2)] ->
+                         In cf (Config C st (m_lete x e1 e2) :: l)) as CONTAINED.
+      { intros; simpl in *; destruct H0; eauto. inversion H0. }
+      pose proof (reach_same FUEL C st e1 [Config C st (m_lete x e1 e2)] (Config C st (m_lete x e1 e2) :: l) CONTAINED) as contra.
+      clear CONTAINED.
+      destruct (eval C st e1 (Config C st (m_lete x e1 e2) :: l) FUEL);
+      destruct (eval C st e1 [Config C st (m_lete x e1 e2)] FUEL);
+      try (rewrite HINT1 in H); try rewrite HINT1';
+      try (simpl in *; destruct H as [[?|?]|?]; eauto; fail);
+      try (inversion contra; fail).
+      destruct contra as [RR [RR' CONTAINED]]. rewrite RR in *. rewrite RR' in *. clear RR RR'.
+      destruct v;
+      try (rewrite HINT1 in H; rewrite HINT1'; destruct H as [[?|?]|?]; simpl in *; eauto). destruct st0.
+      specialize (IHFUEL (C [|dy_c_lete x t ([||])|])
+                         (ST (t !-> ev; mem) (update C (ST mem t) x ev))
+                         e2 reached cf) as HINT2.
+      specialize (IHFUEL (C [|dy_c_lete x t ([||])|])
+                         (ST (t !-> ev; mem) (update C (ST mem t) x ev))
+                         e2 reached0 cf) as HINT2'.
+      pose proof (reach_same FUEL (C [|dy_c_lete x t ([||])|])
+                                  (ST (t !-> ev; mem) (update C (ST mem t) x ev))
+                                  e2 reached0 reached CONTAINED) as contra.
+      clear CONTAINED.
+      destruct (eval (C [|dy_c_lete x t ([||])|])
+                     (ST (t !-> ev; mem) (update C (ST mem t) x ev))
+                     e2 reached FUEL);
+      destruct (eval (C [|dy_c_lete x t ([||])|])
+                     (ST (t !-> ev; mem) (update C (ST mem t) x ev))
+                     e2 reached0 FUEL);
+      try (rewrite HINT2 in H); try rewrite HINT2';
+      try (rewrite HINT1 in H); try rewrite HINT1';
+      try (simpl in *; destruct H as [[[?|?]|?]|?]; eauto; fail);
+      try (inversion contra; fail).
+      destruct contra as [RR [RR' CONTAINED]]. rewrite RR in *. rewrite RR' in *. clear RR RR'.
+      destruct v; rewrite HINT2 in H; try rewrite HINT2';
+      rewrite HINT1 in H; try rewrite HINT1';
+      simpl in *; destruct H as [[[?|?]|?]|?]; eauto.
+    + specialize (IHFUEL C st e1 (Config C st (m_letm M e1 e2) :: l) cf) as HINT1.
+      specialize (IHFUEL C st e1 [Config C st (m_letm M e1 e2)] cf) as HINT1'.
+      assert (forall cf, In cf [Config C st (m_letm M e1 e2)] ->
+                         In cf (Config C st (m_letm M e1 e2) :: l)) as CONTAINED.
+      { intros; simpl in *; destruct H0; eauto. inversion H0. }
+      pose proof (reach_same FUEL C st e1 [Config C st (m_letm M e1 e2)] (Config C st (m_letm M e1 e2) :: l) CONTAINED) as contra.
+      clear CONTAINED.
+      destruct (eval C st e1 (Config C st (m_letm M e1 e2) :: l) FUEL);
+      destruct (eval C st e1 [Config C st (m_letm M e1 e2)] FUEL);
+      try (rewrite HINT1 in H); try rewrite HINT1';
+      try (simpl in *; destruct H as [[?|?]|?]; eauto; fail);
+      try (inversion contra; fail).
+      destruct contra as [RR [RR' CONTAINED]]. rewrite RR in *. rewrite RR' in *. clear RR RR'.
+      destruct v;
+      try (rewrite HINT1 in H; rewrite HINT1'; destruct H as [[?|?]|?]; simpl in *; eauto).
+      specialize (IHFUEL (C [|dy_c_letm M mv ([||])|]) st0 e2 reached cf) as HINT2.
+      specialize (IHFUEL (C [|dy_c_letm M mv ([||])|]) st0 e2 reached0 cf) as HINT2'.
+      pose proof (reach_same FUEL (C [|dy_c_letm M mv ([||])|]) st0 e2 reached0 reached CONTAINED) as contra.
+      clear CONTAINED.
+      destruct (eval (C [|dy_c_letm M mv ([||])|]) st0 e2 reached FUEL);
+      destruct (eval (C [|dy_c_letm M mv ([||])|]) st0 e2 reached0 FUEL);
+      try (rewrite HINT2 in H); try rewrite HINT2';
+      try (rewrite HINT1 in H); try rewrite HINT1';
+      try (simpl in *; destruct H as [[[?|?]|?]|?]; eauto; fail);
+      try (inversion contra; fail).
+      destruct contra as [RR [RR' CONTAINED]]. rewrite RR in *. rewrite RR' in *. clear RR RR'.
+      destruct v; rewrite HINT2 in H; rewrite HINT2';
+      rewrite HINT1 in H; rewrite HINT1';
+      simpl in *; destruct H as [[[?|?]|?]|?]; eauto.
+  - destruct e.
+    + destruct (addr_x C x); destruct st; destruct (mem t); simpl in *; destruct H as [?|[?|?]]; eauto; inversion H.
+    + simpl in *; destruct H as [?|[?|?]]; eauto; inversion H.
+    + specialize (IHFUEL C st e1 (Config C st (e_app e1 e2) :: l) cf) as HINT1'.
+      specialize (IHFUEL C st e1 [Config C st (e_app e1 e2)] cf) as HINT1.
+      assert (forall cf, In cf [Config C st (e_app e1 e2)] ->
+                         In cf (Config C st (e_app e1 e2) :: l)) as CONTAINED.
+      { intros; simpl in *; destruct H0; eauto. inversion H0. }
+      pose proof (reach_same FUEL C st e1 [Config C st (e_app e1 e2)] (Config C st (e_app e1 e2) :: l) CONTAINED) as contra.
+      clear CONTAINED.
+      destruct (eval C st e1 (Config C st (e_app e1 e2) :: l) FUEL);
+      destruct (eval C st e1 [Config C st (e_app e1 e2)] FUEL);
+      try (rewrite HINT1 in H); try rewrite HINT1';
+      try (simpl in *; destruct H as [?|[[?|?]|?]]; eauto; inversion H; fail);
+      try (inversion contra; fail).
+      destruct contra as [RR [RR' CONTAINED]]. rewrite RR in *. rewrite RR' in *. clear RR RR'.
+      destruct v;
+      try (rewrite HINT1 in H; rewrite HINT1'; destruct H as [?|[[?|?]|?]]; simpl in *; eauto; inversion H).
+      destruct ev. simpl in *.
+      specialize (IHFUEL C st0 e2 reached cf) as HINT2'.
+      specialize (IHFUEL C st0 e2 reached0 cf) as HINT2.
+      pose proof (reach_same FUEL C st0 e2 reached0 reached CONTAINED) as contra.
+      clear CONTAINED.
+      destruct (eval C st0 e2 reached FUEL);
+      destruct (eval C st0 e2 reached0 FUEL);
+      try (rewrite HINT2 in H); try rewrite HINT2';
+      try (rewrite HINT1 in H); try rewrite HINT1';
+      try (simpl in *; destruct H as [?|[[[?|?]|?]|?]]; eauto; inversion H; fail);
+      try (inversion contra; fail).
+      destruct contra as [RR [RR' CONTAINED]]. rewrite RR in *. rewrite RR' in *. clear RR RR'.
+      destruct v;
+      try (rewrite HINT2 in H; rewrite HINT2'; rewrite HINT1 in H; rewrite HINT1';
+          destruct H as [?|[[[?|?]|?]|?]]; simpl in *; eauto; inversion H).
+      destruct st2.
+      specialize (IHFUEL (C0 [|dy_c_lam x t ([||])|])
+                         (ST (t !-> ev; mem) (update C (ST mem t) x ev)) 
+                         e reached1 cf) as HINT3'.
+      specialize (IHFUEL (C0 [|dy_c_lam x t ([||])|])
+                         (ST (t !-> ev; mem) (update C (ST mem t) x ev)) 
+                         e reached2 cf) as HINT3.
+      pose proof (reach_same FUEL (C0 [|dy_c_lam x t ([||])|])
+                                  (ST (t !-> ev; mem) (update C (ST mem t) x ev))
+                                  e reached2 reached1 CONTAINED) as contra. clear CONTAINED.
+      destruct (eval (C0 [|dy_c_lam x t ([||])|])
+                     (ST (t !-> ev; mem) (update C (ST mem t) x ev)) e
+                     reached1 FUEL);
+      destruct (eval (C0 [|dy_c_lam x t ([||])|])
+                     (ST (t !-> ev; mem) (update C (ST mem t) x ev)) e
+                     reached2 FUEL);
+      try (rewrite HINT3 in H); try rewrite HINT3';
+      try (rewrite HINT2 in H); try rewrite HINT2';
+      try (rewrite HINT1 in H); try rewrite HINT1';
+      try (simpl in *; destruct H as [?|[[[[?|?]|?]|?]|?]]; eauto 7; inversion H; fail);
+      try (inversion contra; fail).
+      destruct contra as [RR [RR' CONTAINED]]. rewrite RR in *. rewrite RR' in *. clear RR RR'.
+      destruct v; simpl in *;
+      rewrite HINT3 in H; rewrite HINT3';
+      rewrite HINT2 in H; rewrite HINT2';
+      rewrite HINT1 in H; rewrite HINT1';
+      destruct H as [?|[[[[?|?]|?]|?]|?]]; eauto 7; inversion H.
+    + specialize (IHFUEL C st e1 (Config C st (e_link e1 e2) :: l) cf) as HINT1'.
+      specialize (IHFUEL C st e1 [Config C st (e_link e1 e2)] cf) as HINT1.
+      assert (forall cf, In cf [Config C st (e_link e1 e2)] ->
+                         In cf (Config C st (e_link e1 e2) :: l)) as CONTAINED.
+      { intros; simpl in *; destruct H0; eauto. inversion H0. }
+      pose proof (reach_same FUEL C st e1 [Config C st (e_link e1 e2)] (Config C st (e_link e1 e2) :: l) CONTAINED) as contra.
+      clear CONTAINED.
+      destruct (eval C st e1 (Config C st (e_link e1 e2) :: l) FUEL);
+      destruct (eval C st e1 [Config C st (e_link e1 e2)] FUEL);
+      try (rewrite HINT1 in H); try rewrite HINT1';
+      try (simpl in *; destruct H as [?|[[?|?]|?]]; eauto; inversion H; fail);
+      try (inversion contra; fail).
+      destruct contra as [RR [RR' CONTAINED]]. rewrite RR in *. rewrite RR' in *. clear RR RR'.
+      destruct v;
+      try (rewrite HINT1 in H; rewrite HINT1'; destruct H as [?|[[?|?]|?]]; simpl in *; eauto; inversion H).
+      specialize (IHFUEL mv st0 e2 reached cf) as HINT2'.
+      specialize (IHFUEL mv st0 e2 reached0 cf) as HINT2.
+      pose proof (reach_same FUEL mv st0 e2 reached0 reached CONTAINED) as contra.
+      clear CONTAINED.
+      destruct (eval mv st0 e2 reached FUEL);
+      destruct (eval mv st0 e2 reached0 FUEL);
+      try (rewrite HINT2 in H); try rewrite HINT2';
+      try (rewrite HINT1 in H); try rewrite HINT1';
+      try (simpl in *; destruct H as [?|[[[?|?]|?]|?]]; eauto; inversion H; fail);
+      try (inversion contra; fail).
+    + simpl in *. destruct H as [?|[?|?]]; eauto; inversion H.
+    + destruct (ctx_M C M); simpl in *; destruct H as [?|[?|?]]; eauto; inversion H.
+    + specialize (IHFUEL C st e1 (Config C st (m_lete x e1 e2) :: l) cf) as HINT1'.
+      specialize (IHFUEL C st e1 [Config C st (m_lete x e1 e2)] cf) as HINT1.
+      assert (forall cf, In cf [Config C st (m_lete x e1 e2)] ->
+                         In cf (Config C st (m_lete x e1 e2) :: l)) as CONTAINED.
+      { intros; simpl in *; destruct H0; eauto. inversion H0. }
+      pose proof (reach_same FUEL C st e1 [Config C st (m_lete x e1 e2)] (Config C st (m_lete x e1 e2) :: l) CONTAINED) as contra.
+      clear CONTAINED.
+      destruct (eval C st e1 (Config C st (m_lete x e1 e2) :: l) FUEL);
+      destruct (eval C st e1 [Config C st (m_lete x e1 e2)] FUEL);
+      try (rewrite HINT1 in H); try rewrite HINT1';
+      try (simpl in *; destruct H as [?|[[?|?]|?]]; eauto; inversion H; fail);
+      try (inversion contra; fail).
+      destruct contra as [RR [RR' CONTAINED]]. rewrite RR in *. rewrite RR' in *. clear RR RR'.
+      destruct v;
+      try (rewrite HINT1 in H; rewrite HINT1'; destruct H as [?|[[?|?]|?]]; simpl in *; eauto; inversion H). destruct st0.
+      specialize (IHFUEL (C [|dy_c_lete x t ([||])|])
+                         (ST (t !-> ev; mem) (update C (ST mem t) x ev))
+                         e2 reached cf) as HINT2'.
+      specialize (IHFUEL (C [|dy_c_lete x t ([||])|])
+                         (ST (t !-> ev; mem) (update C (ST mem t) x ev))
+                         e2 reached0 cf) as HINT2.
+      pose proof (reach_same FUEL (C [|dy_c_lete x t ([||])|])
+                                  (ST (t !-> ev; mem) (update C (ST mem t) x ev))
+                                  e2 reached0 reached CONTAINED) as contra.
+      clear CONTAINED.
+      destruct (eval (C [|dy_c_lete x t ([||])|])
+                     (ST (t !-> ev; mem) (update C (ST mem t) x ev))
+                     e2 reached FUEL);
+      destruct (eval (C [|dy_c_lete x t ([||])|])
+                     (ST (t !-> ev; mem) (update C (ST mem t) x ev))
+                     e2 reached0 FUEL);
+      try (rewrite HINT2 in H); try rewrite HINT2';
+      try (rewrite HINT1 in H); try rewrite HINT1';
+      try (simpl in *; destruct H as [?|[[[?|?]|?]|?]]; eauto; inversion H; fail);
+      try (inversion contra; fail).
+      destruct contra as [RR [RR' CONTAINED]]. rewrite RR in *. rewrite RR' in *. clear RR RR'.
+      destruct v; rewrite HINT2 in H; try rewrite HINT2';
+      rewrite HINT1 in H; try rewrite HINT1';
+      simpl in *; destruct H as [?|[[[?|?]|?]|?]]; eauto; inversion H.
+    + specialize (IHFUEL C st e1 (Config C st (m_letm M e1 e2) :: l) cf) as HINT1'.
+      specialize (IHFUEL C st e1 [Config C st (m_letm M e1 e2)] cf) as HINT1.
+      assert (forall cf, In cf [Config C st (m_letm M e1 e2)] ->
+                         In cf (Config C st (m_letm M e1 e2) :: l)) as CONTAINED.
+      { intros; simpl in *; destruct H0; eauto. inversion H0. }
+      pose proof (reach_same FUEL C st e1 [Config C st (m_letm M e1 e2)] (Config C st (m_letm M e1 e2) :: l) CONTAINED) as contra.
+      clear CONTAINED.
+      destruct (eval C st e1 (Config C st (m_letm M e1 e2) :: l) FUEL);
+      destruct (eval C st e1 [Config C st (m_letm M e1 e2)] FUEL);
+      try (rewrite HINT1 in H); try rewrite HINT1';
+      try (simpl in *; destruct H as [?|[[?|?]|?]]; eauto; inversion H; fail);
+      try (inversion contra; fail).
+      destruct contra as [RR [RR' CONTAINED]]. rewrite RR in *. rewrite RR' in *. clear RR RR'.
+      destruct v;
+      try (rewrite HINT1 in H; rewrite HINT1'; destruct H as [?|[[?|?]|?]]; simpl in *; eauto; inversion H).
+      specialize (IHFUEL (C [|dy_c_letm M mv ([||])|]) st0 e2 reached cf) as HINT2'.
+      specialize (IHFUEL (C [|dy_c_letm M mv ([||])|]) st0 e2 reached0 cf) as HINT2.
+      pose proof (reach_same FUEL (C [|dy_c_letm M mv ([||])|]) st0 e2 reached0 reached CONTAINED) as contra.
+      clear CONTAINED.
+      destruct (eval (C [|dy_c_letm M mv ([||])|]) st0 e2 reached FUEL);
+      destruct (eval (C [|dy_c_letm M mv ([||])|]) st0 e2 reached0 FUEL);
+      try (rewrite HINT2 in H); try rewrite HINT2';
+      try (rewrite HINT1 in H); try rewrite HINT1';
+      try (simpl in *; destruct H as [?|[[[?|?]|?]|?]]; eauto; inversion H; fail);
+      try (inversion contra; fail).
+      destruct contra as [RR [RR' CONTAINED]]. rewrite RR in *. rewrite RR' in *. clear RR RR'.
+      destruct v; rewrite HINT2 in H; rewrite HINT2';
+      rewrite HINT1 in H; rewrite HINT1';
+      simpl in *; destruct H as [?|[[[?|?]|?]|?]]; eauto; inversion H.
+Qed.
+
+Lemma ReachR_well_defined_l :
+  forall `{TIME : time T} (C : @dy_ctx T) st e C' st' e' (R : <| C st e ~> C' st' e' |>),
+    exists FUEL,
+      In (Config C' st' e') (extract_reached (eval C st e [] FUEL)).
+Proof.
+  intros. rename H into ET. rename H0 into OT.
+  induction R.
+  - exists 1. destruct e; simpl; eauto.
+    destruct (addr_x C x); destruct st; destruct (mem t); simpl; eauto.
+    destruct (ctx_M C M); simpl; eauto.
+  - destruct IHR as [FUEL CONTAINED].
+    exists (S FUEL). simpl.
+    destruct (eval C st e1 [Config C st (e_app e1 e2)] FUEL) eqn:EVAL1;
+    try (rewrite <- EVAL1; rewrite separate_reach; eauto).
+    assert (In (Config C' st' e') (extract_reached (Resolved v st0 reached))).
+    { rewrite <- EVAL1; rewrite separate_reach; eauto. }
+    destruct v; simpl in *; eauto. destruct ev.
+    destruct (eval C st0 e2 reached FUEL) eqn:EVAL2;
+    try (rewrite <- EVAL2; rewrite separate_reach; eauto).
+    assert (In (Config C' st' e') (extract_reached (Resolved v st1 reached0))).
+    { rewrite <- EVAL2; rewrite separate_reach; eauto. }
+    destruct v; simpl in *; eauto. destruct st1.
+    destruct (eval (C0 [|dy_c_lam x t ([||])|])
+                   (ST (t !-> ev; mem) (update C (ST mem t) x ev))
+                   e reached0 FUEL) eqn:EVAL3;
+    try (rewrite <- EVAL3; rewrite separate_reach; eauto).
+    assert (In (Config C' st' e') (extract_reached (Resolved v st1 reached1))).
+    { rewrite <- EVAL3; rewrite separate_reach; eauto. }
+    destruct v; simpl in *; eauto.
+  - destruct IHR as [FUEL CONTAINED].
+    pose proof (EvalR_well_defined_l C st e1 [Config C st (e_app e1 e2)] (EVal (Closure x e C_lam)) st_lam FN).
+    destruct H as [FUEL' CONTAINED'].
+    exists (S (Nat.max FUEL FUEL')). simpl.
+    destruct (eval C st e1 [Config C st (e_app e1 e2)] FUEL') eqn:EVAL1;
+    try (inversion CONTAINED'; fail).
+    destruct CONTAINED' as [RR RR']. rewrite <- RR in *. rewrite RR' in *. clear RR RR'.
+    assert (eval C st e1 [Config C st (e_app e1 e2)] (Nat.max FUEL FUEL') = Resolved (EVal (Closure x e C_lam)) st0 reached) as RR.
+    { apply relax_fuel with (FUEL := FUEL'). nia. eauto. }
+    rewrite RR. clear RR.
+    destruct (eval C st0 e2 reached (Nat.max FUEL FUEL')) eqn:EVAL2;
+    try (rewrite <- EVAL2; rewrite separate_reach; right; 
+        apply relax_fuel_reach with (FUEL := FUEL); try nia; eauto).    
+    assert (In (Config C' st' e') (extract_reached (Resolved v0 st1 reached0))).
+    { rewrite <- EVAL2; rewrite separate_reach.
+      right. apply relax_fuel_reach with (FUEL := FUEL). nia. eauto. }
+    destruct v0; simpl in *; eauto. destruct st1.
+    destruct (eval (C_lam [|dy_c_lam x t ([||])|])
+                   (ST (t !-> ev; mem) (update C (ST mem t) x ev))
+                   e reached0 (Nat.max FUEL FUEL')) eqn:EVAL3;
+    try (rewrite <- EVAL3; rewrite separate_reach; eauto).
+    assert (In (Config C' st' e') (extract_reached (Resolved v0 st1 reached1))).
+    { rewrite <- EVAL3; rewrite separate_reach; eauto. }
+    destruct v0; simpl in *; eauto.
+  - destruct IHR as [FUEL CONTAINED].
+    pose proof (EvalR_well_defined_l C st e1 [Config C st (e_app e1 e2)] (EVal (Closure x e C_lam)) st_lam FN).
+    destruct H as [FUEL' CONTAINED'].
+    destruct (eval C st e1 [Config C st (e_app e1 e2)] FUEL') eqn:EVAL1;
+    try (inversion CONTAINED'; fail).
+    destruct CONTAINED' as [RR RR']. rewrite <- RR in *. rewrite <- RR' in *. clear RR RR'.
+    pose proof (EvalR_well_defined_l C st_lam e2 reached (EVal arg) (ST mem t) ARG).
+    destruct H as [FUEL'' CONTAINED''].
+    destruct (eval C st_lam e2 reached FUEL'') eqn:EVAL2;
+    try (inversion CONTAINED''; fail).
+    destruct CONTAINED'' as [RR RR']. rewrite <- RR in *. rewrite <- RR' in *. clear RR RR'.
+    exists (S (Nat.max FUEL (Nat.max FUEL' FUEL''))).
+    simpl.
+    assert (eval C st e1 [Config C st (e_app e1 e2)]
+                (Nat.max FUEL (Nat.max FUEL' FUEL'')) = Resolved (EVal (Closure x e C_lam)) st_lam reached) as RR.
+    { apply relax_fuel with (FUEL := FUEL'). nia. eauto. } 
+    rewrite RR. clear RR.
+    assert (eval C st_lam e2 reached (Nat.max FUEL (Nat.max FUEL' FUEL'')) = Resolved (EVal arg) (ST mem t) reached0) as RR.
+    { apply relax_fuel with (FUEL := FUEL''). nia. eauto. }
+    rewrite RR. clear RR.
+    destruct (eval (C_lam [|dy_c_lam x t ([||])|])
+                   (ST (t !-> arg; mem) (update C (ST mem t) x arg))
+                   e reached0 (Nat.max FUEL (Nat.max FUEL' FUEL''))) eqn:EVAL3;
+    try (rewrite <- EVAL3; apply relax_fuel_reach with (FUEL := FUEL); try nia; eauto;
+         rewrite separate_reach; eauto).
+    assert (In (Config C' st' e') (extract_reached (Resolved v1 st2 reached1))).
+    { rewrite <- EVAL3; rewrite separate_reach; eauto. right.
+      apply relax_fuel_reach with (FUEL := FUEL); try nia; eauto. }
+    destruct v1; simpl in *; eauto.
+  - destruct IHR as [FUEL CONTAINED].
+    exists (S FUEL). simpl.
+    assert (In (Config C' st' e') (extract_reached (eval C st m [Config C st (e_link m e)] FUEL))).
+    { rewrite separate_reach. eauto. }
+    destruct (eval C st m [Config C st (e_link m e)] FUEL) eqn:EVAL; eauto.
+    destruct v; eauto.
+    assert (In (Config C' st' e') (extract_reached (eval mv st0 e reached FUEL))).
+    { rewrite separate_reach. simpl in *. eauto. }
+    destruct (eval mv st0 e reached FUEL) eqn:EVAL2; eauto.
+  - destruct IHR as [FUEL CONTAINED].
+    pose proof (EvalR_well_defined_l C st m [Config C st (e_link m e)] (MVal C_m) st_m MOD).
+    destruct H as [FUEL' CONTAINED'].
+    destruct (eval C st m [Config C st (e_link m e)] FUEL') eqn:EVAL1;
+    try (inversion CONTAINED'; fail).
+    destruct CONTAINED' as [RR RR']. rewrite <- RR in *. rewrite <- RR' in *. clear RR RR'.
+    exists (S (Nat.max FUEL FUEL')).
+    assert (eval C st m [Config C st (e_link m e)] (Nat.max FUEL FUEL') = Resolved (MVal C_m) st_m reached) as RR.
+    { apply relax_fuel with (FUEL := FUEL'). nia. eauto. }
+    simpl. rewrite RR. clear RR.
+    destruct (eval C_m st_m e reached (Nat.max FUEL FUEL')) eqn:EVAL2;
+    try (rewrite <- EVAL2; rewrite separate_reach; right;
+        apply relax_fuel_reach with (FUEL := FUEL); try nia; eauto).
+  - destruct IHR as [FUEL CONTAINED].
+    exists (S FUEL). simpl.
+    destruct (eval C st e [Config C st (m_lete x e m)] FUEL) eqn:EVAL1;
+    try (rewrite <- EVAL1; rewrite separate_reach; eauto).
+    assert (In (Config C' st' e') (extract_reached (Resolved v st0 reached))).
+    { rewrite <- EVAL1; rewrite separate_reach; eauto. }
+    destruct v; simpl in *; eauto. destruct st0.
+    destruct (eval (C [|dy_c_lete x t ([||])|])
+                   (ST (t !-> ev; mem) (update C (ST mem t) x ev))
+                   m reached FUEL) eqn:EVAL2;
+    try (rewrite <- EVAL2; rewrite separate_reach; eauto).
+    assert (In (Config C' st' e') (extract_reached (Resolved v st0 reached0))).
+    { rewrite <- EVAL2; rewrite separate_reach; eauto. }
+    destruct v; simpl in *; eauto.
+  - destruct IHR as [FUEL CONTAINED].
+    pose proof (EvalR_well_defined_l C st e [Config C st (m_lete x e m)] (EVal v) (ST mem t) EVALx).
+    destruct H as [FUEL' CONTAINED'].
+    destruct (eval C st e [Config C st (m_lete x e m)] FUEL') eqn:EVAL1;
+    try (inversion CONTAINED'; fail).
+    destruct CONTAINED' as [RR RR']. rewrite <- RR in *. rewrite <- RR' in *. clear RR RR'.
+    exists (S (Nat.max FUEL FUEL')).
+    assert (eval C st e [Config C st (m_lete x e m)] (Nat.max FUEL FUEL') = Resolved (EVal v) (ST mem t) reached) as RR.
+    { apply relax_fuel with (FUEL := FUEL'). nia. eauto. }
+    simpl. rewrite RR. clear RR.
+    destruct (eval (C [|dy_c_lete x t ([||])|])
+                   (ST (t !-> v; mem) (update C (ST mem t) x v))
+                   m reached (Nat.max FUEL FUEL')) eqn:EVAL2;
+    try (rewrite <- EVAL2; apply relax_fuel_reach with (FUEL := FUEL); try nia; eauto;
+         rewrite separate_reach; eauto).
+    assert (In (Config C' st' e') (extract_reached (Resolved v1 st1 reached0))).
+    { rewrite <- EVAL2; rewrite separate_reach; eauto. right.
+      apply relax_fuel_reach with (FUEL := FUEL); try nia; eauto. }
+    destruct v1; simpl in *; eauto.
+  - destruct IHR as [FUEL CONTAINED].
+    exists (S FUEL). simpl.
+    destruct (eval C st m1 [Config C st (m_letm M m1 m2)] FUEL) eqn:EVAL1;
+    try (rewrite <- EVAL1; rewrite separate_reach; eauto).
+    assert (In (Config C' st' e') (extract_reached (Resolved v st0 reached))).
+    { rewrite <- EVAL1; rewrite separate_reach; eauto. }
+    destruct v; simpl in *; eauto. destruct st0.
+    destruct (eval (C [|dy_c_letm M mv ([||])|]) (ST mem t) m2 reached FUEL) eqn:EVAL2;
+    try (rewrite <- EVAL2; rewrite separate_reach; eauto).
+    assert (In (Config C' st' e') (extract_reached (Resolved v st0 reached0))).
+    { rewrite <- EVAL2; rewrite separate_reach; eauto. }
+    destruct v; simpl in *; eauto.
+  - destruct IHR as [FUEL CONTAINED].
+    pose proof (EvalR_well_defined_l C st m1 [Config C st (m_letm M m1 m2)] (MVal C_M) st_M EVALM).
+    destruct H as [FUEL' CONTAINED'].
+    destruct (eval C st m1 [Config C st (m_letm M m1 m2)] FUEL') eqn:EVAL1;
+    try (inversion CONTAINED'; fail).
+    destruct CONTAINED' as [RR RR']. rewrite <- RR in *. rewrite <- RR' in *. clear RR RR'.
+    exists (S (Nat.max FUEL FUEL')).
+    assert (eval C st m1 [Config C st (m_letm M m1 m2)] (Nat.max FUEL FUEL') = Resolved (MVal C_M) st_M reached) as RR.
+    { apply relax_fuel with (FUEL := FUEL'). nia. eauto. }
+    simpl. rewrite RR. clear RR.
+    destruct (eval (C [|dy_c_letm M C_M ([||])|]) st_M m2 reached (Nat.max FUEL FUEL')) eqn:EVAL2;
+    try (rewrite <- EVAL2; apply relax_fuel_reach with (FUEL := FUEL); try nia; eauto;
+         rewrite separate_reach; eauto).
+    assert (In (Config C' st' e') (extract_reached (Resolved v0 st1 reached0))).
+    { rewrite <- EVAL2; rewrite separate_reach; eauto. right.
+      apply relax_fuel_reach with (FUEL := FUEL); try nia; eauto. }
+    destruct v0; simpl in *; eauto.
+Qed.
+
+Lemma ReachR_well_defined_r :
+  forall `{TIME : time T} FUEL (C : @dy_ctx T) st e C' st' e'
+         (R : In (Config C' st' e') (extract_reached (eval C st e [] FUEL))),
+  <| C st e ~> C' st' e' |>.
+Proof.
+  intros. rename H into ET. rename H0 into OT.
+  revert C st e C' st' e' R.
+  induction FUEL; intros; simpl in *.
+  - destruct R as [R | R]; inversion R; eauto.
+  - destruct e.
+    + destruct (addr_x C x); destruct st; destruct (mem t); simpl in *;
+      destruct R as [R | R]; inversion R; eauto.
+    + simpl in *. destruct R as [R | R]; inversion R; eauto.
+    + destruct (eval C st e1 [Config C st (e_app e1 e2)] FUEL) eqn:EVAL1;
+      try (rewrite <- EVAL1 in R; rewrite separate_reach in R; simpl in *;
+           destruct R as [[R|R]|R]; try inversion R; eauto).
+      destruct v. all:cycle 1.
+      simpl in *. replace reached with (extract_reached (Resolved (MVal mv) st0 reached)) in R by reflexivity.
+      rewrite <- EVAL1 in R. rewrite separate_reach in R. simpl in *.
+      destruct R as [[R|R]|R]; try inversion R; eauto.
+      destruct ev.
+      pose proof (EvalR_well_defined_r FUEL C st e1 [Config C st (e_app e1 e2)] (EVal (Closure x e C0)) st0).
+      rewrite EVAL1 in H. 
+      assert (EvalR C st e1 (EVal (Closure x e C0)) st0) as FN. 
+      eauto. clear H.
+      destruct (eval C st0 e2 reached FUEL) eqn:EVAL2;
+      try (rewrite <- EVAL2 in R; eauto; rewrite separate_reach in R; simpl in *;
+           destruct R as [R|R]; eauto;
+           replace reached with (extract_reached (Resolved (EVal (Closure x e C0)) st0 reached)) in R by reflexivity;
+           rewrite <- EVAL1 in R; rewrite separate_reach in R; simpl in *;
+           destruct R as [[R|R]|R]; try inversion R; eauto).
+      destruct v. all:cycle 1.
+      simpl in *. replace reached0 with (extract_reached (Resolved (MVal mv) st1 reached0)) in R by reflexivity.
+      rewrite <- EVAL2 in R. rewrite separate_reach in R. simpl in *.
+      replace reached with (extract_reached (Resolved (EVal (Closure x e C0)) st0 reached)) in R by reflexivity.
+      rewrite <- EVAL1 in R. rewrite separate_reach in R. simpl in *.
+      destruct R as [[[R|R]|R]|R]; try inversion R; eauto.
+      destruct st1.
+      pose proof (EvalR_well_defined_r FUEL C st0 e2 reached (EVal ev) (ST mem t)).
+      rewrite EVAL2 in H.
+      assert (EvalR C st0 e2 (EVal ev) (ST mem t)) as ARG.
+      eauto. clear H.
+      destruct (eval (C0 [|dy_c_lam x t ([||])|])
+                     (ST (t !-> ev; mem) (update C (ST mem t) x ev))
+                     e reached0 FUEL) eqn:EVAL3;
+      try (rewrite <- EVAL3 in R; eauto; rewrite separate_reach in R; simpl in *;
+           destruct R as [R|R]; eauto;
+           replace reached0 with (extract_reached (Resolved (EVal ev) (ST mem t) reached0)) in R by reflexivity;
+           rewrite <- EVAL2 in R; rewrite separate_reach in R; simpl in *;
+           replace reached with (extract_reached (Resolved (EVal (Closure x e C0)) st0 reached)) in R by reflexivity;
+           rewrite <- EVAL1 in R; rewrite separate_reach in R; simpl in *;
+           destruct R as [[[R|R]|R]|R]; try inversion R; eauto).
+      replace reached1 with (extract_reached (Resolved v st1 reached1)) in R by reflexivity;
+      rewrite <- EVAL3 in R.
+      destruct v; simpl in *; rewrite separate_reach in R;
+      replace reached0 with (extract_reached (Resolved (EVal ev) (ST mem t) reached0)) in R by reflexivity;
+      rewrite <- EVAL2 in R; rewrite separate_reach in R; simpl in *;
+      replace reached with (extract_reached (Resolved (EVal (Closure x e C0)) st0 reached)) in R by reflexivity;
+      rewrite <- EVAL1 in R; rewrite separate_reach in R; simpl in *;
+      destruct R as [[[[R|R]|R]|R]|R]; try inversion R; eauto.
+    + destruct (eval C st e1 [Config C st (e_link e1 e2)] FUEL) eqn:EVAL1;
+      try (rewrite <- EVAL1 in R; rewrite separate_reach in R; simpl in *;
+           destruct R as [[R|R]|R]; try inversion R; eauto).
+      destruct v.
+      simpl in *. replace reached with (extract_reached (Resolved (EVal ev) st0 reached)) in R by reflexivity.
+      rewrite <- EVAL1 in R. rewrite separate_reach in R. simpl in *.
+      destruct R as [[R|R]|R]; try inversion R; eauto.
+      pose proof (EvalR_well_defined_r FUEL C st e1 [Config C st (e_link e1 e2)] (MVal mv) st0).
+      rewrite EVAL1 in H.
+      assert (EvalR C st e1 (MVal mv) st0) as MOD. 
+      eauto. clear H.
+      destruct (eval mv st0 e2 reached FUEL) eqn:EVAL2;
+      try (rewrite <- EVAL2 in R; eauto; rewrite separate_reach in R; simpl in *;
+           destruct R as [R|R]; eauto;
+           replace reached with (extract_reached (Resolved (MVal mv) st0 reached)) in R by reflexivity;
+           rewrite <- EVAL1 in R; rewrite separate_reach in R; simpl in *;
+           destruct R as [[R|R]|R]; try inversion R; eauto).
+    + simpl in *. destruct R as [R|R]; inversion R; eauto.
+    + destruct (ctx_M C M); simpl in *; destruct R as [R|R]; inversion R; eauto.
+    + destruct (eval C st e1 [Config C st (m_lete x e1 e2)] FUEL) eqn:EVAL1;
+      try (rewrite <- EVAL1 in R; rewrite separate_reach in R; simpl in *;
+           destruct R as [[R|R]|R]; try inversion R; eauto).
+      destruct v. all:cycle 1.
+      simpl in *. replace reached with (extract_reached (Resolved (MVal mv) st0 reached)) in R by reflexivity.
+      rewrite <- EVAL1 in R. rewrite separate_reach in R. simpl in *.
+      destruct R as [[R|R]|R]; try inversion R; eauto.
+      destruct ev.
+      pose proof (EvalR_well_defined_r FUEL C st e1 [Config C st (m_lete x e1 e2)] (EVal (Closure x0 e C0)) st0).
+      rewrite EVAL1 in H. 
+      assert (EvalR C st e1 (EVal (Closure x0 e C0)) st0) as EVALx.
+      eauto. clear H. destruct st0.
+      destruct (eval (C [|dy_c_lete x t ([||])|])
+                     (ST (t !-> Closure x0 e C0; mem)
+                         (update C (ST mem t) x (Closure x0 e C0)))
+                     e2 reached FUEL) eqn:EVAL2;
+      try (rewrite <- EVAL2 in R; eauto; rewrite separate_reach in R; simpl in *;
+           destruct R as [R|R]; eauto;
+           replace reached with (extract_reached (Resolved (EVal (Closure x0 e C0)) (ST mem t) reached)) in R by reflexivity;
+           rewrite <- EVAL1 in R; rewrite separate_reach in R; simpl in *;
+           destruct R as [[R|R]|R]; try inversion R; eauto).
+      destruct v; simpl in *;
+      try (replace reached0 with (extract_reached (Resolved (EVal ev) st0 reached0)) in R by reflexivity);
+      try (replace reached0 with (extract_reached (Resolved (MVal mv) st0 reached0)) in R by reflexivity);
+      rewrite <- EVAL2 in R; rewrite separate_reach in R; simpl in *;
+      replace reached with (extract_reached (Resolved (EVal (Closure x0 e C0)) (ST mem t) reached)) in R by reflexivity;
+      rewrite <- EVAL1 in R; rewrite separate_reach in R; simpl in *;
+      destruct R as [[[R|R]|R]|R]; try inversion R; eauto.
+    + destruct (eval C st e1 [Config C st (m_letm M e1 e2)] FUEL) eqn:EVAL1;
+      try (rewrite <- EVAL1 in R; rewrite separate_reach in R; simpl in *;
+           destruct R as [[R|R]|R]; try inversion R; eauto).
+      destruct v.
+      simpl in *. replace reached with (extract_reached (Resolved (EVal ev) st0 reached)) in R by reflexivity.
+      rewrite <- EVAL1 in R. rewrite separate_reach in R. simpl in *.
+      destruct R as [[R|R]|R]; try inversion R; eauto.
+      pose proof (EvalR_well_defined_r FUEL C st e1 [Config C st (m_letm M e1 e2)] (MVal mv) st0).
+      rewrite EVAL1 in H. 
+      assert (EvalR C st e1 (MVal mv) st0) as EVALm.
+      eauto. clear H.
+      destruct (eval (C [|dy_c_letm M mv ([||])|]) st0 e2 reached FUEL) eqn:EVAL2;
+      try (rewrite <- EVAL2 in R; eauto; rewrite separate_reach in R; simpl in *;
+           destruct R as [R|R]; eauto;
+           replace reached with (extract_reached (Resolved (MVal mv) st0 reached)) in R by reflexivity;
+           rewrite <- EVAL1 in R; rewrite separate_reach in R; simpl in *;
+           destruct R as [[R|R]|R]; try inversion R; eauto).
+      destruct v; simpl in *;
+      try (replace reached0 with (extract_reached (Resolved (EVal ev) st1 reached0)) in R by reflexivity);
+      try (replace reached0 with (extract_reached (Resolved (MVal mv0) st1 reached0)) in R by reflexivity);
+      rewrite <- EVAL2 in R; rewrite separate_reach in R; simpl in *;
+      replace reached with (extract_reached (Resolved (MVal mv) st0 reached)) in R by reflexivity;
+      rewrite <- EVAL1 in R; rewrite separate_reach in R; simpl in *;
+      destruct R as [[[R|R]|R]|R]; try inversion R; eauto.
+Qed.
+
+Theorem ReachR_well_defined :
+  forall `{TIME : time T} (C : @dy_ctx T) st e C' st' e',
+    (exists FUEL, In (Config C' st' e') (extract_reached (eval C st e [] FUEL))) <->
+    <| C st e ~> C' st' e' |>.
+Proof.
+  intros. rename H into ET. rename H0 into OT.
+  split; try apply ReachR_well_defined_l.
+  intros. destruct H as [FUEL CONTAINED].
+  apply ReachR_well_defined_r with (FUEL := FUEL). eauto.
+Qed.
+
+Lemma eval_then_reach :
+  forall `{TIME : time T} FUEL C st e,
+    match eval C st e [] FUEL with
+    | Resolved v st' reached =>
+      exists C' e',
+      In (Config C' st' e') reached /\
+      eval C' st' e' [] 1 = Resolved v st' [Config C' st' e']
+    | _ => True
+    end.
+Proof.
+  assert (forall {X} (l : list X) cf, In cf [] -> In cf l) as HINT.
+  simpl; intros; inversion H.
+  intros. rename H into ET. rename H0 into OT.
+  revert C st e. induction FUEL.
+  - intros. simpl. eauto.
+  - intros. destruct e; simpl.
+    + destruct (addr_x C x) eqn:ADDR; destruct st; destruct (mem t) eqn:ACCESS; eauto.
+      exists C. exists (e_var x). split; simpl; eauto.
+      rewrite ADDR. rewrite ACCESS. eauto.
+    + exists C. exists (e_lam x e). eauto.
+    + destruct (eval C st e1 [Config C st (e_app e1 e2)] FUEL) eqn:FN; eauto.
+      destruct v; eauto. destruct ev.
+      destruct (eval C st0 e2 reached FUEL) eqn:ARG; eauto.
+      destruct v; eauto. destruct st1.
+      destruct (eval (C0 [|dy_c_lam x t ([||])|])
+                     (ST (t !-> ev; mem) (update C (ST mem t) x ev))
+                     e reached0 FUEL) eqn:BODY; eauto.
+      destruct v; eauto.
+      pose proof (reach_same FUEL (C0 [|dy_c_lam x t ([||])|])
+                                  (ST (t !-> ev; mem) (update C (ST mem t) x ev))
+                                  e [] reached0 (HINT _ reached0)) as R.
+      rewrite BODY in R.
+      destruct (eval (C0 [|dy_c_lam x t ([||])|])
+                     (ST (t !-> ev; mem) (update C (ST mem t) x ev))
+                     e [] FUEL) eqn:BODY'; try (inversion R; fail).
+      specialize (IHFUEL (C0 [|dy_c_lam x t ([||])|])
+                         (ST (t !-> ev; mem) (update C (ST mem t) x ev))
+                         e). rewrite BODY' in IHFUEL.
+      destruct R as [RR [RR' R]]. rewrite RR in *. rewrite RR' in *. clear RR RR'.
+      destruct IHFUEL as [C' [e' [CONTAINED EVAL]]].
+      exists C'. exists e'. eauto.
+    + destruct (eval C st e1 [Config C st (e_link e1 e2)] FUEL) eqn:MOD; eauto.
+      destruct v; eauto.
+      destruct (eval mv st0 e2 reached FUEL) eqn:BODY; eauto.
+      pose proof (reach_same FUEL mv st0 e2 [] reached (HINT _ reached)) as R.
+      rewrite BODY in R.
+      destruct (eval mv st0 e2 []) eqn:BODY'; try (inversion R; fail).
+      specialize (IHFUEL mv st0 e2). rewrite BODY' in IHFUEL.
+      destruct R as [RR [RR' R]]. rewrite RR in *. rewrite RR' in *. clear RR RR'.
+      destruct IHFUEL as [C' [e' [CONTAINED EVAL]]].
+      exists C'. exists e'. eauto.
+    + exists C. exists m_empty. eauto.
+    + destruct (ctx_M C M) eqn:ACCESS; eauto.
+      exists C. exists (m_var M). rewrite ACCESS. simpl in *; eauto.
+    + destruct (eval C st e1 [Config C st (m_lete x e1 e2)] FUEL) eqn:EVALx; eauto.
+      destruct v; eauto. destruct st0.
+      destruct (eval (C [|dy_c_lete x t ([||])|])
+                     (ST (t !-> ev; mem) (update C (ST mem t) x ev))
+                     e2 reached FUEL) eqn:BODY; eauto.
+      pose proof (reach_same FUEL (C [|dy_c_lete x t ([||])|])
+                                  (ST (t !-> ev; mem) (update C (ST mem t) x ev))
+                                  e2 [] reached (HINT _ reached)) as R.
+      rewrite BODY in R.
+      destruct (eval (C [|dy_c_lete x t ([||])|])
+                     (ST (t !-> ev; mem) (update C (ST mem t) x ev))
+                     e2 []) eqn:BODY'; try (inversion R; fail).
+      specialize (IHFUEL (C [|dy_c_lete x t ([||])|])
+                         (ST (t !-> ev; mem) (update C (ST mem t) x ev))
+                         e2). rewrite BODY' in IHFUEL.
+      destruct R as [RR [RR' R]]. rewrite RR in *. rewrite RR' in *. clear RR RR'.
+      destruct IHFUEL as [C' [e' [CONTAINED EVAL]]].
+      destruct v; eauto.
+    + destruct (eval C st e1 [Config C st (m_letm M e1 e2)] FUEL) eqn:EVALM; eauto.
+      destruct v; eauto.
+      destruct (eval (C [|dy_c_letm M mv ([||])|]) st0 e2 reached FUEL) eqn:BODY; eauto.
+      pose proof (reach_same FUEL (C [|dy_c_letm M mv ([||])|]) st0 e2 [] reached (HINT _ reached)) as R.
+      rewrite BODY in R.
+      destruct (eval (C [|dy_c_letm M mv ([||])|]) st0 e2 []) eqn:BODY'; try (inversion R; fail).
+      specialize (IHFUEL (C [|dy_c_letm M mv ([||])|]) st0 e2). rewrite BODY' in IHFUEL.
+      destruct R as [RR [RR' R]]. rewrite RR in *. rewrite RR' in *. clear RR RR'.
+      destruct IHFUEL as [C' [e' [CONTAINED EVAL]]].
+      destruct v; eauto.
+Qed.
+
+Corollary EvalR_then_ReachR :
+  forall `{TIME : time T} C st e v st'
+         (R : EvalR C st e v st'),
+    exists C' e',
+      <| C st e ~> C' st' e' |> /\
+      eval C' st' e' [] 1 = Resolved v st' [Config C' st' e'].
+Proof.
+  intros. rewrite <- (EvalR_well_defined []) in R.
+  destruct R as [FUEL R].
+  destruct (eval C st e [] FUEL) eqn:EVAL;
+  try (inversion R; fail).
+  destruct R as [RR RR']. rewrite RR in *. rewrite RR' in *. clear RR RR'.
+  pose proof (eval_then_reach FUEL C st e) as EXACT.
+  rewrite EVAL in EXACT. destruct EXACT as [C' [e' [REACH EXACT]]].
+  replace reached with (extract_reached (Resolved v0 st0 reached)) in REACH by reflexivity.
+  rewrite <- EVAL in REACH.
+  assert (<| C st e ~> C' st0 e' |>).
+  { rewrite <- ReachR_well_defined. exists FUEL. eauto. }
+  exists C'. exists e'. eauto.
+Qed. 
 
 Lemma value_reach_only_itself :
   forall `{TIME : time T} C st v (pf : value v)
